documentation of equivalence prices, etc

Ready_simulation.thy
@@ -11,10 +11,10 @@ inductive hml_ready_sim :: "('a, 's) hml \<Rightarrow> bool"
 "hml_ready_sim TT" |
 "hml_ready_sim (hml_pos \<alpha> \<phi>)" if "hml_ready_sim \<phi>" |
 "hml_ready_sim (hml_conj I J \<Phi>)" if 
-"(\<forall>x \<in> (\<Phi> ` I). hml_ready_sim x) \<and> (\<forall>y \<in> (\<Phi> ` J). (\<exists>\<alpha>. y = (hml_pos \<alpha> TT)))"
+"(\<forall>x \<in> (\<Phi> ` I). hml_ready_sim x) \<and> (\<forall>y \<in> (\<Phi> ` J). (\<exists>\<alpha>. y = (hml_pos \<alpha> TT)) \<or> y = TT)"
 
 definition hml_ready_sim_formulas where
-"hml_ready_sim_formulas \<equiv> {\<phi>. hml_ready_sim \<phi>}"
+  "hml_ready_sim_formulas \<equiv> {\<phi>. hml_ready_sim \<phi>}"
 
 definition expr_ready_sim
   where
@@ -107,8 +107,7 @@ next
     by force+
   from 3 have "\<forall>x\<in>\<Phi> ` I. less_eq_t (expr x) (\<infinity>, \<infinity>, \<infinity>, \<infinity>, 1, 1)"
     by blast
-  hence fa_pos: "\<forall>x \<in>\<Phi> ` I.  expr_5 x \<le> 1"
-"\<forall>x \<in>\<Phi> ` I.  expr_6 x \<le> 1"
+  hence fa_pos: "\<forall>x \<in>\<Phi> ` I.  expr_5 x \<le> 1" "\<forall>x \<in>\<Phi> ` I.  expr_6 x \<le> 1"
     using less_eq_t.simps expr.simps 
     by force+
   with fa_neg have e5: "(Sup ((expr_5 \<circ> \<Phi>) ` I \<union> (expr_5 \<circ> \<Phi>) ` J \<union> (expr_1 \<circ> \<Phi>) ` J)) \<le> 1"
@@ -184,48 +183,344 @@ lemma ready_sim_left:
   assumes "less_eq_t (expr \<phi>) (\<infinity>, \<infinity>, \<infinity>, \<infinity>, 1, 1)"
   shows "HML_ready_sim \<phi>"
   using assms
-proof (induction \<phi>)
-  case TT
-  then show ?case 
-    using HML_ready_sim.intros(1) by blast
-next
-  case (hml_pos x1 \<phi>)
-  then show ?case 
-    by (simp add: HML_ready_sim.intros(2)) 
-next
-  case (hml_conj I J \<Phi>)
-  hence "expr_5 (hml_conj I J \<Phi>) \<le> 1"
-"expr_6 (hml_conj I J \<Phi>) \<le> 1"
-    by (metis expr.simps less_eq_t.simps)+
-  hence "Sup ((expr_5 \<circ> \<Phi>) ` I) \<le> 1"
-"Sup ((expr_6 \<circ> \<Phi>) ` I) \<le> 1"
-    using expr_5_conj expr_6.expr_6_conj Sup_union_distrib 
-    by (metis le_sup_iff)+
-  hence "\<forall>x \<in> \<Phi> ` I. expr_5 x \<le> 1"
-"\<forall>x \<in> \<Phi> ` I. expr_6 x \<le> 1"
-    using Sup_le_iff
-    by (metis image_comp image_eqI)+   
-  hence "\<forall>x \<in> \<Phi> ` I. less_eq_t (expr x) (\<infinity>, \<infinity>, \<infinity>, \<infinity>, 1, 1)"
-    by simp
-  hence "\<forall>x \<in> \<Phi> ` I. HML_ready_sim x" using hml_conj
-    by blast
-  have "Sup((expr_5 \<circ> \<Phi>) ` J) \<le> 1" "Sup((expr_1 \<circ> \<Phi>) ` J) \<le> 1"
-    using \<open>expr_5 (hml_conj I J \<Phi>) \<le> 1\<close>
-    by (simp add: Sup_union_distrib)+
-  hence "\<forall>x \<in> \<Phi> ` J. expr_1 x \<le> 1"
-    using Sup_le_iff
-    by (metis image_comp image_eqI)
-  have "Sup((eSuc \<circ> expr_6 \<circ> \<Phi>) ` J) <= 1"
-    using \<open>expr_6 (hml_conj I J \<Phi>) \<le> 1\<close>
-    by (simp add: Sup_union_distrib)
-  hence "Sup((expr_6 \<circ> \<Phi>) ` J) <= 0"
-    by (metis (no_types, opaque_lifting) SUP_image Sup_enat_def eSuc_Sup eSuc_ile_mono one_eSuc zero_le)
-  hence "\<forall>x \<in> \<Phi> ` J. expr_6 x \<le> 0"
-    using Sup_le_iff
-    by (metis image_comp image_eqI)
-  with \<open>\<forall>x \<in> \<Phi> ` J. expr_1 x \<le> 1\<close> have "\<forall>x \<in> \<Phi> ` J. single_pos_pos x"
-    using single_pos_pos_expr by blast
-  then show ?case using \<open>\<forall>x \<in> \<Phi> ` I. HML_ready_sim x\<close> hml_ready_sim.intros(3) 
-    by (meson Ready_simulation.HML_ready_sim.intros(3))
+  proof (induction \<phi>)
+    case TT
+    then show ?case 
+      using HML_ready_sim.intros(1) by blast
+  next
+    case (hml_pos x1 \<phi>)
+    then show ?case 
+      by (simp add: HML_ready_sim.intros(2)) 
+  next
+    case (hml_conj I J \<Phi>)
+    hence "expr_5 (hml_conj I J \<Phi>) \<le> 1"
+  "expr_6 (hml_conj I J \<Phi>) \<le> 1"
+      by (metis expr.simps less_eq_t.simps)+
+    hence "Sup ((expr_5 \<circ> \<Phi>) ` I) \<le> 1"
+  "Sup ((expr_6 \<circ> \<Phi>) ` I) \<le> 1"
+      using expr_5_conj expr_6.expr_6_conj Sup_union_distrib 
+      by (metis le_sup_iff)+
+    hence "\<forall>x \<in> \<Phi> ` I. expr_5 x \<le> 1" "\<forall>x \<in> \<Phi> ` I. expr_6 x \<le> 1"
+      using Sup_le_iff
+      by (metis image_comp image_eqI)+   
+    hence "\<forall>x \<in> \<Phi> ` I. less_eq_t (expr x) (\<infinity>, \<infinity>, \<infinity>, \<infinity>, 1, 1)"
+      by simp
+    hence "\<forall>x \<in> \<Phi> ` I. HML_ready_sim x" using hml_conj
+      by blast
+    have "Sup((expr_5 \<circ> \<Phi>) ` J) \<le> 1" "Sup((expr_1 \<circ> \<Phi>) ` J) \<le> 1"
+      using \<open>expr_5 (hml_conj I J \<Phi>) \<le> 1\<close>
+      by (simp add: Sup_union_distrib)+
+    hence "\<forall>x \<in> \<Phi> ` J. expr_1 x \<le> 1"
+      using Sup_le_iff
+      by (metis image_comp image_eqI)
+    have "Sup((eSuc \<circ> expr_6 \<circ> \<Phi>) ` J) <= 1"
+      using \<open>expr_6 (hml_conj I J \<Phi>) \<le> 1\<close>
+      by (simp add: Sup_union_distrib)
+    hence "Sup((expr_6 \<circ> \<Phi>) ` J) <= 0"
+      by (metis (no_types, opaque_lifting) SUP_image Sup_enat_def eSuc_Sup eSuc_ile_mono one_eSuc zero_le)
+    hence "\<forall>x \<in> \<Phi> ` J. expr_6 x \<le> 0"
+      using Sup_le_iff
+      by (metis image_comp image_eqI)
+    with \<open>\<forall>x \<in> \<Phi> ` J. expr_1 x \<le> 1\<close> have "\<forall>x \<in> \<Phi> ` J. single_pos_pos x"
+      using single_pos_pos_expr by blast
+    then show ?case using \<open>\<forall>x \<in> \<Phi> ` I. HML_ready_sim x\<close> hml_ready_sim.intros(3) 
+      by (meson Ready_simulation.HML_ready_sim.intros(3))
 qed
+
+context lts begin
+
+lemma alt_single_pos_pos:
+  fixes s::'s
+  assumes "single_pos_pos \<phi>" "\<not> HML_true \<phi>"
+  shows "\<forall>s. \<exists>I \<Phi>. 
+          (s \<Turnstile> \<phi>) = (s \<Turnstile> (hml_conj I {} \<Phi>)) \<and> (\<forall>\<psi> \<in> \<Phi> ` I. (\<exists>\<alpha>. \<psi> = hml_pos \<alpha> TT))"
+  using assms proof(induct)
+  case 1
+  then show ?case 
+    using TT_like.intros(1) lts.HML_true_TT_like 
+    by auto
+next
+  case (2 \<psi> \<alpha>)
+  hence "HML_true \<psi>" 
+    using HML_true_nested_empty_pos_conj by blast
+  define \<Psi> where "\<Psi> \<equiv> (\<lambda>i. (if i = s then (hml_pos \<alpha> TT)::('a, 's)hml else undefined))"
+  hence "\<forall>t. (t \<Turnstile> (hml_pos \<alpha> \<psi>)) = (t \<Turnstile> (hml_conj {s} {} \<Psi>))" 
+    using HML_true_def \<open>HML_true \<psi>\<close> by auto 
+  hence "\<forall>t. (t \<Turnstile> hml_pos \<alpha> \<psi>) = (t \<Turnstile> hml_conj {s} {} \<Psi>) \<and> (\<forall>\<psi>\<in>\<Psi> ` {s}. \<exists>\<alpha>. \<psi> = hml_pos \<alpha> TT)"
+    using HML_true_def \<Psi>_def \<open>HML_true \<psi>\<close> by force
+  then show ?case by blast
+next
+  case (3 \<Phi> I J)
+  show "\<forall>s. \<exists>Ia \<Phi>'.
+              (s \<Turnstile> hml_conj I J \<Phi>) = (s \<Turnstile> hml_conj Ia {} \<Phi>') \<and> (\<forall>\<psi>\<in>\<Phi>' ` Ia. \<exists>\<alpha>. \<psi> = hml_pos \<alpha> TT)"
+  proof
+    fix s::'s
+    define Is where "Is \<equiv> {t. (\<exists>\<alpha>. t \<in> derivatives t \<alpha>)}"
+      
+  show "\<exists>Ia \<Phi>'.
+          (s \<Turnstile> hml_conj I J \<Phi>) = (s \<Turnstile> hml_conj Ia {} \<Phi>') \<and> (\<forall>\<psi>\<in>\<Phi>' ` Ia. \<exists>\<alpha>. \<psi> = hml_pos \<alpha> TT)"
+    sorry
+  
+  qed
+qed
+
+lemma single_pos_pos_equiv_to_pos_conj:
+  fixes s::'s
+  assumes "single_pos_pos \<phi>" "\<not>HML_true \<phi>"
+  shows "\<exists>I \<Phi>. (\<forall>s. (s \<Turnstile> \<phi>) = (s \<Turnstile> (hml_conj I {} \<Phi>)) \<and> (\<forall>\<psi> \<in> \<Phi> ` I. \<exists>\<alpha>. \<psi> = hml_pos \<alpha> TT))"
+  using assms proof(induct)
+  case 1
+  then show ?case 
+    using TT_like.intros(1) lts.HML_true_TT_like by blast
+next
+  case (2 \<psi> \<alpha>)
+  hence "HML_true \<psi>" 
+    using HML_true_nested_empty_pos_conj by blast
+  define \<Psi> where "\<Psi> \<equiv> (\<lambda>i. (if i = s then (hml_pos \<alpha> TT)::('a, 's)hml else undefined))"
+  hence "\<forall>t. (t \<Turnstile> (hml_pos \<alpha> \<psi>)) = (t \<Turnstile> (hml_conj {s} {} \<Psi>))" 
+    using HML_true_def \<open>HML_true \<psi>\<close> by auto 
+  hence "\<forall>t. (t \<Turnstile> hml_pos \<alpha> \<psi>) = (t \<Turnstile> hml_conj {s} {} \<Psi>) \<and> (\<forall>\<psi>\<in>\<Psi> ` {s}. \<exists>\<alpha>. \<psi> = hml_pos \<alpha> TT)"
+    using HML_true_def \<Psi>_def \<open>HML_true \<psi>\<close> by force
+  then show ?case by blast
+next
+  case (3 \<Phi> I J)
+  have "\<forall>s. (s \<Turnstile> (hml_conj I J \<Phi>)) = (s \<Turnstile> (hml_conj (I-{i. HML_true (\<Phi> i)}) J \<Phi>))" 
+    using DiffD1 DiffI HML_true_def by auto
+  define reach_der where "reach_der \<equiv> {s. \<exists>t \<alpha>. s \<in> derivatives t \<alpha>}"
+  define univ_set where "univ_set \<equiv> {x::'s.True}"
+  define pos_set where "pos_set \<equiv> {\<psi>. \<exists>\<phi> \<in> \<Phi> ` I. \<exists>I' \<Phi>'. \<forall>s. (s \<Turnstile> \<phi>) = (s \<Turnstile> (hml_conj I' {} \<Phi>'))
+                                                                 \<and> \<psi> \<in> \<Phi>' ` I'}"
+  have "(\<nexists>f::'s \<Rightarrow>('a, 's)hml. \<forall>x \<in> pos_set. \<exists>i \<in> univ_set. f i = x) 
+          \<longrightarrow> (\<forall>s. \<not> s \<Turnstile> (hml_conj I J \<Phi>))"
+  proof
+    assume "\<nexists>f. \<forall>x\<in>pos_set. \<exists>i\<in>univ_set. f i = x"
+    show "\<forall>s. \<not> s \<Turnstile> hml_conj I J \<Phi>" proof
+      fix t ::'s
+      {
+        assume "t \<Turnstile> (hml_conj I J \<Phi>)"
+        have "\<exists>f::'s \<Rightarrow> ('a, 's) hml. \<forall>x \<in> pos_set. \<exists>i \<in> univ_set. f i = x" 
+        proof-
+          have "I \<union> J \<subseteq> univ_set"
+            unfolding univ_set_def by blast
+
+          have "\<forall>x \<in> pos_set. \<exists>i \<in> univ_set. \<Phi> i = x" sorry
+        proof(rule ccontr)
+      }
+  qed
+  show " \<exists>Ia \<Phi>'.
+          \<forall>s. (s \<Turnstile> hml_conj I J \<Phi>) = (s \<Turnstile> hml_conj Ia {} \<Phi>') \<and> (\<forall>\<psi>\<in>\<Phi>' ` Ia. \<exists>\<alpha>. \<psi> = hml_pos \<alpha> TT) "
+  proof(cases "(\<nexists>f::'s \<Rightarrow>('a, 's)hml. \<forall>x \<in> pos_set. \<exists>i \<in> reach_der. f i = x)")
+    case True
+    then show ?thesis sorry
+  next
+    case False
+    then obtain f where "\<forall>x\<in>pos_set. \<exists>i\<in>reach_der. f i = x" by blast
+    have "\<forall>s. (s \<Turnstile> hml_conj I J \<Phi>) = (s \<Turnstile> hml_conj reach_der {} f) \<and> (\<forall>\<psi>\<in>f ` reach_der. \<exists>\<alpha>. \<psi> = hml_pos \<alpha> TT)"
+    sorry
+    then show ?thesis sorry
+  qed
+  
+  define Indexunion where "Indexunion \<equiv> {J. (\<exists>\<phi> \<in> \<Phi> ` I. (\<exists>\<Phi>. \<forall>s. (s \<Turnstile> \<phi>) = (s \<Turnstile> hml_conj I {} \<Phi>) \<and> (\<forall>\<psi>\<in>\<Phi> ` I. \<exists>\<alpha>. \<psi> = hml_pos \<alpha> TT)))}"
+  have "card Indexunion \<ge> card "
+  have ""
+  consider "\<forall>I' J'. "
+  then show ?case sorry
+qed
+
+lemma alt_ready_sim_implies_ready_sim:
+  fixes \<phi> :: "('a, 's) hml"
+  assumes "hml_ready_sim \<phi>"
+  shows "\<exists>\<psi>. HML_ready_sim \<psi> \<and> (\<forall>s. (s \<Turnstile> \<phi>) \<longleftrightarrow> (s \<Turnstile> \<psi>))"
+  using assms proof induct
+  case 1
+  then show ?case 
+    using Ready_simulation.HML_ready_sim.intros(1) by blast
+next
+  case (2 \<phi> \<alpha>)
+  then obtain \<psi> where "HML_ready_sim \<psi>" "(\<forall>s. (s \<Turnstile> \<phi>) = (s \<Turnstile> \<psi>))" by blast
+  hence "HML_ready_sim (hml_pos \<alpha> \<psi>)" 
+    using Ready_simulation.HML_ready_sim.simps by blast
+  then show ?case 
+    by (meson \<open>\<forall>s. (s \<Turnstile> \<phi>) = (s \<Turnstile> \<psi>)\<close> hml_sem_pos)
+next
+  case (3 \<Phi> I J)
+  consider "I \<inter> J = {} \<and> (\<forall>y\<in>\<Phi> ` J. \<exists>\<alpha>. y = hml_pos \<alpha> TT)" 
+    | "(\<exists>i. i \<in> (I \<inter> J)) \<and> (\<forall>y\<in>\<Phi> ` J. \<exists>\<alpha>. y = hml_pos \<alpha> TT)" 
+    | "(\<exists>j \<in> J. \<Phi> j = TT)"
+    using "3" by blast
+  then show ?case proof(cases)
+    case 1
+    hence "(\<forall>y\<in>\<Phi> ` J. \<exists>\<alpha>. y = hml_pos \<alpha> TT)" 
+      using "3"
+      by simp
+    have "\<forall>\<alpha>. single_pos_pos (hml_pos \<alpha> TT)" 
+      using Ready_traces.single_pos_pos.simps nested_empty_pos_conj.intros(1) by blast
+    define \<Psi> where "\<Psi> \<equiv> (\<lambda>i. (if i \<in> I
+                            then (SOME \<psi>. HML_ready_sim \<psi> \<and> (\<forall>s. (s \<Turnstile> \<Phi> i) = (s \<Turnstile> \<psi>))) 
+                            else (if i \<in> J then \<Phi> i else undefined)))"
+    have "\<forall>j \<in> I. \<exists>\<psi>. HML_ready_sim \<psi> \<and> (\<forall>s. (s \<Turnstile> \<Phi> j) = (s \<Turnstile> \<psi>))"
+      using "3" by blast
+    hence "\<forall>i\<in> I. \<exists>\<psi>. \<Psi> i = \<psi> \<and> HML_ready_sim \<psi> \<and> (\<forall>s. (s \<Turnstile> \<Phi> i) = (s \<Turnstile> \<psi>))" 
+      unfolding \<Psi>_def someI_ex
+      by (smt (verit) someI_ex)
+    hence "\<forall>j \<in> I. \<forall>s. (s \<Turnstile> \<Phi> j) = (s \<Turnstile> \<Psi> j)" 
+      using "3" "1" Ready_simulation.HML_ready_sim.intros image_iff \<Psi>_def 
+      by blast
+    have "\<forall>i \<in> J. \<forall>s. (s \<Turnstile> \<Phi> i) = (s \<Turnstile> \<Psi> i)"
+      using "1" "3"
+      unfolding \<Psi>_def 
+      by force
+    have "\<forall>i \<in> J. single_pos_pos (\<Psi> i)"
+      unfolding \<Psi>_def
+      using "1" "3" \<open>\<forall>\<alpha>. Ready_traces.single_pos_pos (hml_pos \<alpha> TT)\<close>
+      by fastforce
+    hence "HML_ready_sim (hml_conj I J \<Psi>)" 
+      using \<open>\<forall>j \<in> I. \<exists>\<psi>. HML_ready_sim \<psi> \<and> (\<forall>s. (s \<Turnstile> \<Phi> j) = (s \<Turnstile> \<psi>))\<close> 
+      by (metis (mono_tags, lifting) Ready_simulation.HML_ready_sim.intros(3) \<open>\<forall>i\<in>I. \<exists>\<psi>. \<Psi> i = \<psi> \<and> Ready_simulation.HML_ready_sim \<psi> \<and> (\<forall>s. (s \<Turnstile> \<Phi> i) = (s \<Turnstile> \<psi>))\<close> image_iff)
+    have "(\<forall>s. (s \<Turnstile> hml_conj I J \<Phi>) = (s \<Turnstile> (hml_conj I J \<Psi>)))"
+      by (simp add: \<open>\<forall>i\<in>J. \<forall>s. (s \<Turnstile> \<Phi> i) = (s \<Turnstile> \<Psi> i)\<close> \<open>\<forall>j\<in>I. \<forall>s. (s \<Turnstile> \<Phi> j) = (s \<Turnstile> \<Psi> j)\<close>)
+    then show ?thesis 
+      using "1" HML_ready_sim.intros(1) \<open>\<forall>j \<in> I. \<forall>s. (s \<Turnstile> \<Phi> j) = (s \<Turnstile> \<Psi> j)\<close> \<open>Ready_simulation.HML_ready_sim (hml_conj I J \<Psi>)\<close> by blast
+  next
+    case 2
+    assume  "(\<exists>i. i \<in> I \<inter> J) \<and> (\<forall>y\<in>\<Phi> ` J. \<exists>\<alpha>. y = hml_pos \<alpha> TT)"
+      then obtain i where "i \<in> I \<inter> J" by blast
+      hence "\<forall>s. \<not>((s \<Turnstile> (\<Phi> i)) \<and> (\<not>(s \<Turnstile> (\<Phi> i))))" 
+        by blast
+      hence "\<forall>s. \<not>((\<forall>i \<in> I. s \<Turnstile> (\<Phi> i)) \<and> (\<forall>j \<in> J. \<not>(s \<Turnstile> (\<Phi> j))))"
+        using \<open>i \<in> I \<inter> J\<close> by blast
+      hence "\<forall>s. \<not>s\<Turnstile>(hml_conj I J \<Phi>)" 
+        using hml_sem_conj by presburger
+      have "single_pos_pos (\<Phi> i)"
+        using \<open>i \<in> I \<inter> J\<close> "3"
+        using "2" Ready_traces.single_pos_pos.intros(2) nested_empty_pos_conj.intros(1) by fastforce
+      hence "HML_ready_sim (\<Phi> i)" 
+        using "3" Ready_simulation.HML_ready_sim.intros(1) Ready_simulation.HML_ready_sim.intros(2) \<open>i \<in> I \<inter> J\<close> by fastforce
+      hence "HML_ready_sim (hml_conj {i} {i} \<Phi>)" 
+        using \<open>single_pos_pos (\<Phi> i) \<close>
+        by (simp add: Ready_simulation.HML_ready_sim.intros(3))
+      have "\<forall>s. \<not>s\<Turnstile>(hml_conj {i} {i} \<Phi>)" 
+        by simp
+      then show ?thesis 
+        using \<open>Ready_simulation.HML_ready_sim (hml_conj {i} {i} \<Phi>)\<close> \<open>\<forall>s. \<not> s \<Turnstile> hml_conj I J \<Phi>\<close> by blast
+    next
+      case 3
+      assume "\<exists>j\<in>J. \<Phi> j = TT"
+      then obtain j where "j\<in> J" "\<Phi> j = TT" by blast
+      hence "\<forall>s. \<not>s\<Turnstile>(hml_conj I J \<Phi>)" 
+        by fastforce
+      have "HML_ready_sim (hml_conj {} {j} \<Phi>)" 
+        by (smt (verit, del_insts) Ready_simulation.HML_ready_sim.intros(3) Ready_traces.single_pos_pos.simps \<open>\<Phi> j = TT\<close> ball_empty image_empty image_insert insert_iff)
+      have "\<forall>s. \<not>s\<Turnstile>(hml_conj {} {j} \<Phi>)" 
+        by (simp add: \<open>\<Phi> j = TT\<close>)
+      then show ?thesis using \<open>HML_ready_sim (hml_conj {} {j} \<Phi>)\<close> 
+        using \<open>\<forall>s. \<not> s \<Turnstile> hml_conj I J \<Phi>\<close> by blast
+    qed
+qed
+
+lemma ready_sim_implies_alt_ready_sim:
+fixes \<phi> :: "('a, 's) hml"
+  assumes "HML_ready_sim \<phi>"
+  shows "\<exists>\<psi>. hml_ready_sim \<psi> \<and> (\<forall>s. (s \<Turnstile> \<phi>) \<longleftrightarrow> (s \<Turnstile> \<psi>))"
+  using assms proof induct
+  case 1
+  then show ?case 
+    using hml_ready_sim.intros(1) by blast
+next
+  case (2 \<phi> \<alpha>)
+  then obtain \<psi> where "hml_ready_sim \<psi>" "(\<forall>s. (s \<Turnstile> \<phi>) = (s \<Turnstile> \<psi>))" by blast
+  hence "hml_ready_sim (hml_pos \<alpha> \<psi>)" 
+    using Ready_simulation.hml_ready_sim.simps by blast
+  then show ?case 
+    by (meson \<open>\<forall>s. (s \<Turnstile> \<phi>) = (s \<Turnstile> \<psi>)\<close> hml_sem_pos)
+next
+  case (3 \<Phi> I J)
+  consider "I \<inter> J = {} \<and> (\<forall>y\<in>\<Phi> ` J. single_pos_pos y \<and> \<not>HML_true y)" 
+    | "(\<exists>i. i \<in> (I \<inter> J))" 
+    | "(\<exists>j \<in> J. HML_true (\<Phi> j))"
+    using "3" by blast
+  then show ?case proof(cases)
+    case 1
+    hence "(\<forall>y\<in>\<Phi> ` J. \<exists>\<alpha>. (\<forall>s. (s \<Turnstile> y) = (s \<Turnstile> (hml_pos \<alpha> TT))))" 
+      using "3" single_pos_pos_equiv_to_pos by blast
+    have "\<forall>\<alpha>. single_pos_pos (hml_pos \<alpha> TT)" 
+      using Ready_traces.single_pos_pos.simps nested_empty_pos_conj.intros(1) by blast
+    define \<Psi> where "\<Psi> \<equiv> (\<lambda>i. (if i \<in> I
+                            then (SOME \<psi>. hml_ready_sim \<psi> \<and> (\<forall>s. (s \<Turnstile> \<Phi> i) = (s \<Turnstile> \<psi>))) 
+                            else (if i \<in> J then (hml_pos (SOME \<alpha>. (\<forall>s. (s \<Turnstile> (\<Phi> i)) = (s \<Turnstile> (hml_pos \<alpha> TT)))) TT) else undefined)))"
+    have "\<forall>j \<in> I. \<exists>\<psi>. hml_ready_sim \<psi> \<and> (\<forall>s. (s \<Turnstile> \<Phi> j) = (s \<Turnstile> \<psi>))"
+      using "3" by blast
+    hence "\<forall>i\<in> I. \<exists>\<psi>. \<Psi> i = \<psi> \<and> hml_ready_sim \<psi> \<and> (\<forall>s. (s \<Turnstile> \<Phi> i) = (s \<Turnstile> \<psi>))" 
+      unfolding \<Psi>_def someI_ex
+      by (smt (verit) someI_ex)
+    hence "\<forall>j \<in> I. \<forall>s. (s \<Turnstile> \<Phi> j) = (s \<Turnstile> \<Psi> j)" 
+      using "3" "1" Ready_simulation.HML_ready_sim.intros image_iff \<Psi>_def 
+      by blast
+    have "\<forall>i \<in> J. \<exists>\<alpha>. \<Psi> i = (hml_pos \<alpha> TT)"
+      using "1" "3" \<open>(\<forall>y\<in>\<Phi> ` J. \<exists>\<alpha>. (\<forall>s. (s \<Turnstile> y) = (s \<Turnstile> (hml_pos \<alpha> TT))))\<close> someI_ex
+      unfolding \<Psi>_def
+      by auto
+    hence "\<forall>i \<in> J. \<Psi> i = (hml_pos (SOME \<alpha>. (\<forall>s. (s \<Turnstile> (\<Phi> i)) = (s \<Turnstile> (hml_pos \<alpha> TT)))) TT)"
+      unfolding \<Psi>_def 
+      using "1" by auto 
+    have "\<forall>i \<in> J. \<forall>s. (s \<Turnstile> \<Phi> i) = (s \<Turnstile> \<Psi> i)" 
+      proof
+      fix i
+      assume "i \<in> J"
+      then show "\<forall>s. (s \<Turnstile> \<Phi> i) = (s \<Turnstile> \<Psi> i)" proof-
+        have "\<Psi> i = (hml_pos (SOME \<alpha>. (\<forall>s. (s \<Turnstile> (\<Phi> i)) = (s \<Turnstile> (hml_pos \<alpha> TT)))) TT)"
+        using \<open>\<forall>i\<in>J. \<Psi> i = hml_pos (SOME \<alpha>. \<forall>s. (s \<Turnstile> \<Phi> i) = (s \<Turnstile> hml_pos \<alpha> TT)) TT\<close> \<open>i \<in> J\<close> by blast
+      then obtain \<alpha> where "\<Psi> i = (hml_pos \<alpha> TT)"
+        by blast
+      hence "\<forall>s. (s \<Turnstile> \<Phi> i) = (s \<Turnstile> hml_pos \<alpha> TT)" 
+        by (smt (verit, ccfv_threshold) \<open>\<Psi> i = hml_pos (SOME \<alpha>. \<forall>s. (s \<Turnstile> \<Phi> i) = (s \<Turnstile> hml_pos \<alpha> TT)) TT\<close> \<open>\<forall>y\<in>\<Phi> ` J. \<exists>\<alpha>. \<forall>s. (s \<Turnstile> y) = (s \<Turnstile> hml_pos \<alpha> TT)\<close> \<open>i \<in> J\<close> image_iff someI_ex)
+      hence "\<forall>s. (s \<Turnstile> \<Phi> i) = (s \<Turnstile> \<Psi> i)" 
+        using \<open>\<Psi> i = hml_pos \<alpha> TT\<close> by presburger
+      then show "\<forall>s. (s \<Turnstile> \<Phi> i) = (s \<Turnstile> \<Psi> i)" by blast
+    qed
+  qed
+    have "\<forall>i \<in> J. \<exists>\<alpha>. (\<Psi> i) = hml_pos \<alpha> TT"
+      unfolding \<Psi>_def
+      using "1" "3" \<open>\<forall>\<alpha>. Ready_traces.single_pos_pos (hml_pos \<alpha> TT)\<close> by fastforce
+    hence "hml_ready_sim (hml_conj I J \<Psi>)" 
+      using \<open>\<forall>j \<in> I. \<exists>\<psi>. hml_ready_sim \<psi> \<and> (\<forall>s. (s \<Turnstile> \<Phi> j) = (s \<Turnstile> \<psi>))\<close> Ready_simulation.HML_ready_sim.intros(3) \<open>\<forall>i\<in>I. \<exists>\<psi>. \<Psi> i = \<psi> \<and> hml_ready_sim \<psi> \<and> (\<forall>s. (s \<Turnstile> \<Phi> i) = (s \<Turnstile> \<psi>))\<close> image_iff
+      by (simp add: hml_ready_sim.intros(3))
+    have "(\<forall>s. (s \<Turnstile> hml_conj I J \<Phi>) = (s \<Turnstile> (hml_conj I J \<Psi>)))"
+      by (simp add: \<open>\<forall>i\<in>J. \<forall>s. (s \<Turnstile> \<Phi> i) = (s \<Turnstile> \<Psi> i)\<close> \<open>\<forall>j\<in>I. \<forall>s. (s \<Turnstile> \<Phi> j) = (s \<Turnstile> \<Psi> j)\<close>)
+    then show ?thesis 
+      using "1" HML_ready_sim.intros(1) \<open>\<forall>j \<in> I. \<forall>s. (s \<Turnstile> \<Phi> j) = (s \<Turnstile> \<Psi> j)\<close> \<open>hml_ready_sim (hml_conj I J \<Psi>)\<close> by blast
+  next
+    case 2
+    assume  "(\<exists>i. i \<in> I \<inter> J)"
+    then obtain i where "i \<in> I \<inter> J" by blast
+    hence "\<forall>s. \<not>((s \<Turnstile> (\<Phi> i)) \<and> (\<not>(s \<Turnstile> (\<Phi> i))))" 
+      by blast
+    hence "\<forall>s. \<not>((\<forall>i \<in> I. s \<Turnstile> (\<Phi> i)) \<and> (\<forall>j \<in> J. \<not>(s \<Turnstile> (\<Phi> j))))"
+      using \<open>i \<in> I \<inter> J\<close> by blast
+    hence "\<forall>s. \<not>s\<Turnstile>(hml_conj I J \<Phi>)" 
+      using hml_sem_conj by presburger
+    define \<Psi> where "\<Psi> \<equiv> (\<lambda>j. (if j = i then TT::('a, 's)hml else undefined))"
+    hence "hml_ready_sim (hml_conj {i} {i} \<Psi>)" 
+      by (smt (verit) hml_ready_sim.simps image_empty image_insert singletonD)
+    have "\<forall>s. \<not>s\<Turnstile>(hml_conj {i} {i} \<Psi>)" 
+      by simp
+    then show ?thesis 
+      using \<open>\<forall>s. \<not> s \<Turnstile> hml_conj I J \<Phi>\<close> \<open>hml_ready_sim (hml_conj {i} {i} \<Psi>)\<close> by blast
+  next
+    assume "\<exists>j\<in>J. HML_true (\<Phi> j)"
+    hence "\<forall>s. \<not>(s\<Turnstile>(hml_conj I J \<Phi>))" 
+      using HML_true_def by force
+    obtain j where "j\<in>J" "HML_true (\<Phi> j)" 
+      using \<open>\<exists>j\<in>J. HML_true (\<Phi> j)\<close> by blast
+    define \<Psi> where "\<Psi> \<equiv> (\<lambda>i. (if i = j then TT::('a, 's)hml else undefined))"
+    have "hml_ready_sim (hml_conj {} {j} \<Psi>)" 
+      by (simp add: \<Psi>_def hml_ready_sim.intros(3))
+    have "\<forall>s. \<not>(s\<Turnstile>(hml_conj {} {j} \<Psi>))" 
+      by (simp add: \<Psi>_def)
+    then show ?thesis using \<open>hml_ready_sim (hml_conj {} {j} \<Psi>)\<close> 
+      using \<open>\<forall>s. \<not> s \<Turnstile> hml_conj I J \<Phi>\<close> by blast
+  qed
+qed
+
+end
 end
