formula_prices_list.thy
@@ -8,86 +8,15 @@ begin
 
 section \<open>Price Spectra of Behavioral Equivalences\<close>
 
-text \<open>The linear-time--branching-time spectrum can be represented in terms of HML-expressiveness (s.h. section HML).
-(Deciding all at once)(energy games) show how one can think of the amount of HML-expressiveness used by a formula by its \textit{price}.
-The equivalences of the spectrum (or their modal-logical characterizations) can then be defined in terms of \textit{price coordinates}, that is
-equivalence $X$ is characterized by the HML formulas with prices less then or equal to a \textit{X-price bound} $e_X$.
-We use the six dimensions from (energy games) to characterize the notions of equivalence we are interested in (In figure xx oder so umschreiben).
-Intuitively, the dimensions can be described as follows:\\
-1. Formula modal depth of observations: How many modal operations $\langle \alpha \rangle$ may one pass when descending the syntax tree. (Algebraic laws for nondeterminism and concurrency)(Operational and algebraic semantics of concurrent processes)\\
-2. Formula nesting depth of conjunctions: How often may one pass a conjunction?\\
-3. Maximal modal depth of deepest positive clauses in conjunctions\\
-4. Maximal modal depth of other positive clauses in conjunctions\\
-5. Maximal modal depth of negative clauses in conjunctions\\
-6. Formula nesting depth of negations\\\<close>
+text \<open>\cite{bisping2023process, bisping2022deciding} use a pricing system to measure the amount of HML-expressiveness used by a formula. By assigning an expressiveness price to each formula, the authors create a price lattice that allows for comparing distinguishing power of different formulas, where lower prices indicate less distinguishing power. This allows for a new way of defining HML-subsets. Instead of bounding the subsets by the structure of the included formulas, they are defined as sets of formulas whose prices are less than or equal to a given expressiveness price bound, or \textit{price coordinates}.
+The value of each dimension of these price coordinates constrains different syntactic features of the formulas. The authors derive the linear-time--branching-time spectrum by assigning a price coordinate to every equivalence in the spectrum, see \cref{fig:1_1}. In this section, we introduce the definition of the expressiveness price function of (\cite{bisping2023process}, definition 5) and how that function is used to chart the spectrum.\<close>
+
+text \<open>Unlike \cite{bisping2023process}, we define the price for every dimension $i$ as a seperate function, $\textsf{expr}_i : \text{HML}[\Sigma] \rightarrow (\mathbb{N \cup \{\infty\}})$ and combine them to the expressiveness function, $\textsf{expr} : \text{HML}[\Sigma] \rightarrow (\mathbb{N \cup \{\infty\}})^6$. Each function inductively traverses the syntax tree of a formula and increases its value when encountering the respective syntax feature.\<close>
 
 subsubsection \<open>Definition 2.3.1 (Formula Prices)\<close>
-text \<open>
-The expressiveness price $\textsf{expr} : \text{HML}[\Sigma] \rightarrow (\mathbb{N \cup \infty})^6$ of a formula interpreted as $6 \times 1$-dimensional vectors is defined recursively by:
-
-\[
-\text{expr}(\langle a \rangle \varphi) :=
-\begin{pmatrix}
-1 + \text{expr}_1(\varphi) \\
-\text{expr}_2(\varphi) \\
-\text{expr}_3(\varphi) \\
-\text{expr}_4(\varphi) \\
-\text{expr}_5(\varphi) \\
-\text{expr}_6(\varphi) \\
-\end{pmatrix}
-\]
-
-\[
-\text{expr}(\neg \varphi) := 
-\begin{pmatrix}
-\text{expr}_1(\varphi) \\
-\text{expr}_2(\varphi) \\
-\text{expr}_3(\varphi) \\
-\text{expr}_4(\varphi) \\
-\text{expr}_5(\varphi) \\
-1 + \text{expr}_6(\varphi) \\
-\end{pmatrix}
-\]
-
-\[
-\text{expr}\left( \bigwedge_{i \in I} \psi_i \right) := \sup(\{
-\begin{pmatrix}
-0 \\
-1 + \sup_{i \in I} \text{expr}_2(\psi_i) \\
-\sup_{i \in \text{Pos}} \text{expr}_1(\psi_i) \\
-\sup_{i \in \text{Pos} \backslash \mathcal{R}} \text{expr}_1(\psi_i) \\
-\sup_{i \in \text{Neg}} \text{expr}_1(\psi_i) \\
-0 \\
-\end{pmatrix} \} \cup \{\textsf{expr}(\psi_i) | i \in I\} 
-\]
-
-where:
-
-$\textit{Neg} := \{i \in I \, | \, \exists \varphi'_i. \psi_i = \neg \varphi'_i\}$
-
-$\textit{Pos} := I \setminus \text{Neg}$
-
-$\mathcal{R} := \left\{
-\begin{aligned}
-&\varnothing \text{ if } \textit{Pos} = \varnothing, \\
-&\{ r \} \text{ for some } r \in \textit{Pos} \text{ where } \text{expr}_1(\psi_r) \text{ maximal for \textit{Pos}}
-\end{aligned}
-\right.$
-
-Our Isabelle definition of HML makes it very easy to derive the sets Pos and Neg, by \<open>\<Phi> ` I\<close> and \<open>\<Phi> ` J\<close> respectively.
-
-Remark: We deviate from the definition in (cite Bisp) by including infinity in the domain of the function due to infinite branching conjunctions. Supremum over infinite set wird zu unendlich.\<close>
-
-text \<open>To better argue about the function we define each dimension as a seperate function.\<close>
-
-text \<open>Vlt als erstes: modaltiefe als beispiel für observation expressiveness von formel, mit isabelle definition,
-dann pos\_r definition,
-direct\_expr definition,
-einzelne dimensionen,
-lemma direct\_expr = expr...\<close>
-
-text \<open>Formally, the \textit{modal depth} $\textsf{expr}_1$ of a formula $\varphi$ is defined recursively by:
-
+text \<open>\textit{
+(\textcolor{red}{1}) The \textnormal{modal depth} $\textsf{expr}_1$ measures the nesting depth of observations within a formula: $\text{HML}[\Sigma] \rightarrow (\mathbb{N} \cup \{\infty\})$ of a formula $\varphi$ is defined recursively by:}
+\textit{
 \begin{align*}
     \text{if } \varphi &= \langle a \rangle \psi \quad \text{ with } a \in \Sigma \\
     &\text{then } \textsf{expr}_1(\varphi) = 1 + \textsf{expr}_1(\psi) \\
@@ -96,7 +25,101 @@ text \<open>Formally, the \textit{modal depth} $\textsf{expr}_1$ of a formula $\
     \text{if } \psi &= \neg \varphi \\
     &\text{then } \textsf{expr}_1(\psi) = \textsf{expr}_1(\varphi)
 \end{align*}
+}
+
+
+\textit{(\textcolor{orange}{2}) The \textnormal{nesting depth of conjunctions} $\textsf{expr}_2$ measures the maximal number of conjunctions that are nested inside one another in a formula: $\text{HML}[\Sigma] \rightarrow (\mathbb{N} \cup \{\infty\})$ of a formula $\varphi$ is defined recursively by:}
+\textit{
+\begin{align*}
+    \text{if } \varphi &= \langle a \rangle \psi \quad \text{ with } a \in \Sigma \\
+    & \text{then } \textsf{expr}_2(\varphi) = \textsf{expr}_2(\psi) \\
+    \text{if } \varphi &= \bigwedge_{i \in I} \{\psi_i \} \\
+    & \text{then } \textsf{expr}_2(\varphi) = 1 + \sup(\textsf{expr}_2(\psi_i)) \\
+    \text{if } \psi &= \neg \varphi \\
+    & \text{then } \textsf{expr}_2(\psi) = \textsf{expr}_2(\varphi)
+\end{align*}
+}
+
+\textit{(\textcolor{myyellow}{3}) The \textnormal{maximal modal depth of deepest positive clauses in conjunctions} $\textsf{expr}_3$ measures the deepest modal depth of the positive conjuncts of all conjunctions of a formula: $\text{HML}[\Sigma] \rightarrow (\mathbb{N} \cup \{\infty\})$ of a formula $\varphi$ is defined recursively by:}
+
+\textit{\begin{align*}
+    \text{if } \varphi &= \langle a \rangle \psi \quad \text{ with } a \in \Sigma \\
+    & \text{then } \textsf{md}(\varphi) = \textsf{md}(\psi) \\
+    \text{if } \varphi &= \bigwedge_{i \in I} \{ \psi_i \} \\
+    & \text{then } \textsf{md}(\varphi) = \sup(\{\textsf{expr}_1(\psi_i) | i \in \text{Pos}\} \cup \{\textsf{expr}_3(\psi_i) | i \in I\}) \\
+    \text{if } \psi &= \neg \varphi \\
+    & \text{then } \textsf{expr}_3(\psi) = \textsf{expr}_3(\varphi)
+\end{align*}
+}
+
+\textit{(\textcolor{green}{4}) The \textnormal{maximal modal depth of other positive clauses in conjunctions} $\textsf{expr}_4$ measures the deepest positive modal depth aside from the deepest positive clause: $\text{HML}[\Sigma] \rightarrow (\mathbb{N} \cup \{\infty\})$ of a formula $\varphi$ is defined recursively by:}
+\textit{
+\begin{align*}
+    \text{if } \varphi &= \langle a \rangle \psi \quad \text{ with } a \in \Sigma \\
+    & \text{then } \textsf{expr}_4(\varphi) = \textsf{expr}_4(\psi) \\
+    \text{if } \varphi &= \bigwedge_{i \in I} \{\ \psi_i \} \\
+    & \text{then } \text{md}(\varphi) = \sup(\{\textsf{expr}_1(\psi_i)|i\in\text{Pos}\backslash \mathcal{R}\}\cup\{\textsf{expr}_4(\psi_i) | i \in I\}) \\
+    \text{if } \psi &= \neg \varphi \\
+    & \text{then } \textsf{expr}_4(\psi) = \textsf{expr}_4(\varphi)
+\end{align*}
+}
+
+\textit{
+(\textcolor{cyan}{5}) The \textnormal{maximal modal depth of negative clauses in conjunctions} $\textsf{expr}_5$ measures the deepest modal depth of the negative conjuncts of all conjunctions of a formula: $\text{HML}[\Sigma] \rightarrow (\mathbb{N} \cup \{\infty\})$ of a formula $\varphi$ is defined recursively by:
+}
+\textit{
+\begin{align*}
+    \text{if } \varphi &= \langle a \rangle \psi \quad \text{ with } a \in \Sigma \\
+    & \text{then } \textsf{expr}_5(\varphi) = \textsf{expr}_5(\psi) \\
+    \text{if } \varphi &= \bigwedge_{i \in I} \{ \psi_i \} \\
+    & \text{then } \textsf{expr}_5(\varphi) = \sup(\{\textsf{expr}_1(\psi_i)| i \in \text{Neg}\}\cup \{\textsf{expr}_5(\psi_i)|i \in I\}) \\
+    \text{if } \psi &= \neg \varphi \\
+    & \text{then } \textsf{expr}_5(\psi) = \textsf{expr}_5(\varphi)
+\end{align*}
+}
+\textit{(\textcolor{violet}{6}) The \textnormal{nesting depth of negations} $\textsf{expr}_{6}$ measures the maximal number of negations when traversing the syntax tree of a formula: $\text{HML}[\Sigma] \rightarrow (\mathbb{N} \cup \{\infty\})$ of a formula $\varphi$ is defined recursively by:}
+\textit{
+\begin{align*}
+    \text{if } \varphi &= \langle a \rangle \psi \quad \text{ with } a \in \Sigma \\
+    & \text{then } \textsf{expr}_6(\varphi) = \textsf{expr}_6(\psi) \\
+    \text{if } \varphi &= \bigwedge_{i \in I} \{ \psi_i \} \\
+    & \text{then } \textsf{expr}_6(\varphi) = \sup(\{\textsf{expr}_6(\psi_i)| i \in I\}) \\
+    \text{if } \psi &= \neg \varphi \\
+    & \text{then } \textsf{expr}_6(\psi) = 1 + \textsf{expr}_6(\varphi)
+\end{align*}
+}
+\textit{where:}
+
+$\textit{Neg} := \{i \in I \, | \, \exists \varphi'_i. \psi_i = \neg \varphi'_i\}$
+
+$\textit{Pos} := I \setminus \text{Neg}$
+
+$\mathcal{R} := \left\{
+\begin{aligned}
+&\varnothing \textit{ if } \textit{Pos} = \varnothing, \\
+&\{ r \} \textit{ for some } r \in \textit{Pos} \text{ where } \textit{expr}_1(\psi_r) \textit{ maximal for \textit{Pos}}
+\end{aligned}
+\right\}.$
+
+\textit{We combine this to the expressiveness price $\textsf{expr}: \text{HML}[\Sigma] \rightarrow (\mathbb{N \cup \infty})^6$ of a formula $\varphi$:
+\[
+\text{expr}(\varphi) :=
+\begin{pmatrix}
+\text{expr}_1(\varphi) \\
+\text{expr}_2(\varphi) \\
+\text{expr}_3(\varphi) \\
+\text{expr}_4(\varphi) \\
+\text{expr}_5(\varphi) \\
+\text{expr}_6(\varphi) \\
+\end{pmatrix}
+\]
+}
+
+We show that $\textsf{expr}$ defines the same function as (\cite{bisping2023process}, definition 5) in (appendix).
 \<close>
+
+text \<open>The formalization closely follows the structure outlined in the definition. Neg and Pos can easily be derived using our formalization of Conjunctions. \\
+The function \<open>pos_r\<close> formalizes the set $Pos - \mathcal{R}$. It invokes the axiom of choice by selecting and removing a formula with maximal modal depth from Pos using the Hilbert choice operator \<open>SOME\<close>.\<close>
 
 primrec expr_1 :: "('a, 's)hml \<Rightarrow> enat"
   where
@@ -105,7 +128,17 @@ expr_1_conj: \<open>expr_1 (hml_conj I J \<Phi>) = Sup ((expr_1 \<circ> \<Phi>) 
 expr_1_pos: \<open>expr_1 (hml_pos \<alpha> \<phi>) = 
   1 + (expr_1 \<phi>)\<close>
 
-text \<open>With the help of the modal depth we can derive Pos$\backslash$R in Isabelle:\<close>
+primrec expr_2 :: "('a, 's)hml \<Rightarrow> enat"
+  where
+expr_2_tt: \<open>expr_2 TT = 1\<close> |
+expr_2_conj: \<open>expr_2 (hml_conj I J \<Phi>) = 1 + Sup ((expr_2 \<circ> \<Phi>) ` I \<union> (expr_2 \<circ> \<Phi>) ` J)\<close> |
+expr_2_pos: \<open>expr_2 (hml_pos \<alpha> \<phi>) = expr_2 \<phi>\<close>
+
+primrec expr_3 :: "('a, 's) hml \<Rightarrow> enat"
+  where
+expr_3_tt: \<open>expr_3 TT = 0\<close> |
+expr_3_pos: \<open>expr_3 (hml_pos \<alpha> \<phi>) = expr_3 \<phi>\<close> | 
+expr_3_conj: \<open>expr_3 (hml_conj I J \<Phi>) = (Sup ((expr_1 \<circ> \<Phi>) ` I \<union> (expr_3 \<circ> \<Phi>) ` I \<union> (expr_3 \<circ> \<Phi>) ` J))\<close>
 
 fun pos_r :: "('a, 's)hml set \<Rightarrow> ('a, 's)hml set"
   where
@@ -115,136 +148,11 @@ let max_val = (Sup (expr_1 ` xs));
   xs_new = xs - {max_elem}
 in xs_new)"
 
-text \<open>Now we can directly define the expressiveness function as \<open>direct_expr\<close>.\<close>
-
-function direct_expr :: "('a, 's)hml \<Rightarrow> enat \<times> enat \<times> enat \<times> enat \<times> enat \<times> enat" where
-  "direct_expr TT = (0, 1, 0, 0, 0, 0)" |
-  "direct_expr (hml_pos \<alpha> \<phi>) = (1 + fst (direct_expr \<phi>), 
-                                fst (snd (direct_expr \<phi>)), 
-                                fst (snd (snd (direct_expr \<phi>))), 
-                                fst (snd (snd (snd (direct_expr \<phi>)))), 
-                                fst (snd (snd (snd (snd (direct_expr \<phi>))))), 
-                                snd (snd (snd (snd (snd (direct_expr \<phi>))))))" |
-  "direct_expr (hml_conj I J \<Phi>) = (Sup ((fst \<circ> direct_expr \<circ> \<Phi>) ` I \<union> (fst \<circ> direct_expr \<circ> \<Phi>) ` J), 
-                                    1 + Sup ((fst \<circ> snd \<circ> direct_expr \<circ> \<Phi>) ` I \<union> (fst \<circ> snd \<circ> direct_expr \<circ> \<Phi>) ` J), 
-(Sup ((fst \<circ> direct_expr \<circ> \<Phi>) ` I \<union> (fst \<circ> snd \<circ> snd \<circ> direct_expr \<circ> \<Phi>) ` I \<union> (fst \<circ> snd \<circ> snd \<circ> direct_expr \<circ> \<Phi>) ` J)),
-(Sup (((fst \<circ> direct_expr) ` (pos_r (\<Phi> ` I)))  \<union> (fst \<circ> snd \<circ> snd \<circ> snd \<circ> direct_expr \<circ> \<Phi>) ` I \<union> (fst \<circ> snd \<circ> snd \<circ> snd \<circ> direct_expr \<circ> \<Phi>) ` J)),  
-(Sup ((fst \<circ> snd \<circ> snd \<circ> snd \<circ> snd \<circ> direct_expr \<circ> \<Phi>) ` I \<union> (fst \<circ> snd \<circ> snd \<circ> snd \<circ> snd \<circ> direct_expr \<circ> \<Phi>) ` J \<union> (fst \<circ> direct_expr \<circ> \<Phi>) ` J)), 
-(Sup ((snd \<circ> snd \<circ> snd \<circ> snd \<circ> snd \<circ> direct_expr \<circ> \<Phi>) ` I \<union> ((eSuc \<circ> snd \<circ> snd \<circ> snd \<circ> snd \<circ> snd \<circ> direct_expr \<circ> \<Phi>) ` J))))"
-  by ((meson hml.exhaust), simp+)
-
-text \<open>In order to demonstrate termination of the function, it is necessary to establish that each sequence of recursive function calls reaches a base case. 
-This is accomplished by proving that the relation between process-formula pairs, as defined recursively by the function, is contained within a well-founded relation. 
-A relation \( R \subset X \times X \) is considered well-founded if every non-empty subset \( X' \subset X \) contains a minimal element \( m \) such that \( (x, m) \notin R \) for all \( x \in X' \). 
-A key property of well-founded relations is that all descending chains \( (x_0, x_1, x_2, \ldots) \) (where \( (x_i, x_{i+1}) \in R \)) originating from any element \( x_0 \in X \) are finite. 
-Consequently, this ensures that each sequence of recursive invocations terminates after a finite number of steps. 
-
-These proofs were inspired by the Isabelle formalizations presented in [WEP+16].
-\<close>
-
-inductive_set HML_wf_rel :: "(('a, 's)hml) rel" where
-"\<phi> = \<Phi> i \<and> i \<in> (I \<union> J) \<Longrightarrow> (\<phi>, (hml_conj I J \<Phi>)) \<in> HML_wf_rel" |
-"(\<phi>, (hml_pos \<alpha> \<phi>)) \<in> HML_wf_rel"
-
-lemma HML_wf_rel_is_wf: \<open>wf HML_wf_rel\<close>
-  unfolding wf_def
-proof safe
-  fix P
-  assume assm: "\<forall>x. (\<forall>y. (y, x) \<in> HML_wf_rel \<longrightarrow> P y) \<longrightarrow> P x"
-  show "\<And>\<phi>. P \<phi>" proof-
-    fix \<phi>
-    show "P \<phi>" proof(induction \<phi>)
-    case TT
-    then show ?case 
-      using HML_wf_rel.cases assm by blast
-  next
-    case (hml_pos x1 \<phi>)
-    then show ?case 
-      using HML_wf_rel.cases hml.inject hml.simps assm 
-      by (smt (verit, best))
-  next
-    case (hml_conj x1 x2 x3)
-    then show ?case 
-      using assm
-      by (metis HML_wf_rel.cases hml.inject(2) hml.simps(8) rangeI)
-    qed
-  qed
-qed
-
-lemma pos_r_subs: "pos_r (\<Phi> ` I) \<subseteq> (\<Phi> ` I)"
-  by auto
-
-termination
-  apply rule
-  using HML_wf_rel_is_wf HML_wf_rel.simps Un_iff pos_r_subs by fastforce+
-
-text \<open>The other functions are also defined recursively:
-
-Formula nesting depth of conjunctions $\textsf{expr}_2$:
-
-\begin{align*}
-    \text{if } \varphi &= \langle a \rangle \psi \quad \text{ with } a \in \Sigma \\
-    & \text{then } \textsf{expr}_2(\varphi) = \textsf{expr}_2(\psi) \\
-    \text{if } \varphi &= \bigwedge_{i \in I} \{\psi_i \} \\
-    & \text{then } \textsf{expr}_2(\varphi) = 1 + \sup(\textsf{expr}_2(\psi_i)) \\
-    \text{if } \psi &= \neg \varphi \\
-    & \text{then } \textsf{expr}_2(\psi) = \textsf{expr}_2(\varphi)
-\end{align*}
-\<close>
-
-primrec expr_2 :: "('a, 's)hml \<Rightarrow> enat"
-  where
-expr_2_tt: \<open>expr_2 TT = 1\<close> |
-expr_2_conj: \<open>expr_2 (hml_conj I J \<Phi>) = 1 + Sup ((expr_2 \<circ> \<Phi>) ` I \<union> (expr_2 \<circ> \<Phi>) ` J)\<close> |
-expr_2_pos: \<open>expr_2 (hml_pos \<alpha> \<phi>) = expr_2 \<phi>\<close>
-
-text \<open>Maximal modal depth of the deepest positive branch $\textsf{expr}_3$:
-
-\begin{align*}
-    \text{if } \varphi &= \langle a \rangle \psi \quad \text{ with } a \in \Sigma \\
-    & \text{then } \textsf{md}(\varphi) = \textsf{md}(\psi) \\
-    \text{if } \varphi &= \bigwedge_{i \in I} \{ \psi_i \} \\
-    & \text{then } \textsf{md}(\varphi) = \sup(\{\textsf{expr}_1(\psi_i) | i \in \text{Pos}\} \cup \{\textsf{expr}_3(\psi_i) | i \in I\}) \\
-    \text{if } \psi &= \neg \varphi \\
-    & \text{then } \textsf{expr}_3(\psi) = \textsf{expr}_3(\varphi)
-\end{align*}
-\<close>
-
-primrec expr_3 :: "('a, 's) hml \<Rightarrow> enat"
-  where
-expr_3_tt: \<open>expr_3 TT = 0\<close> |
- expr_3_pos: \<open>expr_3 (hml_pos \<alpha> \<phi>) = expr_3 \<phi>\<close> | 
-expr_3_conj: \<open>expr_3 (hml_conj I J \<Phi>) = (Sup ((expr_1 \<circ> \<Phi>) ` I \<union> (expr_3 \<circ> \<Phi>) ` I \<union> (expr_3 \<circ> \<Phi>) ` J))\<close>
-
-text \<open>Maximal modal depth of other positive clauses in conjunctions $\textsf{expr}_4$:
-
-\begin{align*}
-    \text{if } \varphi &= \langle a \rangle \psi \quad \text{ with } a \in \Sigma \\
-    & \text{then } \textsf{expr}_4(\varphi) = \textsf{expr}_4(\psi) \\
-    \text{if } \varphi &= \bigwedge_{i \in I} \{\ \psi_i \} \\
-    & \text{then } \text{md}(\varphi) = \sup(\{\textsf{expr}_1(\psi_i)|i\in\text{Pos}\backslash \mathcal{R}\}\cup\{\textsf{expr}_4(\psi_i) | i \in I\}) \\
-    \text{if } \psi &= \neg \varphi \\
-    & \text{then } \textsf{expr}_4(\psi) = \textsf{expr}_4(\varphi)
-\end{align*}
-\<close>
-
 primrec expr_4 :: "('a, 's)hml \<Rightarrow> enat" 
   where
 expr_4_tt: "expr_4 TT = 0" |
 expr_4_pos: "expr_4 (hml_pos a \<phi>) = expr_4 \<phi>" |
 expr_4_conj: "expr_4 (hml_conj I J \<Phi>) = Sup ((expr_1 ` (pos_r (\<Phi> ` I)))  \<union> (expr_4 \<circ> \<Phi>) ` I \<union> (expr_4 \<circ> \<Phi>) ` J)"
-
-text \<open>Maximal modal depth of negative clauses in conjunctions $\textsf{expr}_5$:
-
-\begin{align*}
-    \text{if } \varphi &= \langle a \rangle \psi \quad \text{ with } a \in \Sigma \\
-    & \text{then } \textsf{expr}_5(\varphi) = \textsf{expr}_5(\psi) \\
-    \text{if } \varphi &= \bigwedge_{i \in I} \{ \psi_i \} \\
-    & \text{then } \textsf{expr}_5(\varphi) = \sup(\{\textsf{expr}_1(\psi_i)| i \in \text{Neg}\}\cup \{\textsf{expr}_5(\psi_i)|i \in I\}) \\
-    \text{if } \psi &= \neg \varphi \\
-    & \text{then } \textsf{expr}_5(\psi) = \textsf{expr}_5(\varphi)
-\end{align*}
-\<close>
 
 primrec expr_5 :: "('a, 's)hml \<Rightarrow> enat"
   where
@@ -253,18 +161,6 @@ expr_5_pos:\<open>expr_5 (hml_pos \<alpha> \<phi>) = expr_5 \<phi>\<close>|
 expr_5_conj: \<open>expr_5 (hml_conj I J \<Phi>) = 
 (Sup ((expr_5 \<circ> \<Phi>) ` I \<union> (expr_5 \<circ> \<Phi>) ` J \<union> (expr_1 \<circ> \<Phi>) ` J))\<close>
 
-text \<open>Formula nesting depth of negations $\textsf{expr}_6$:
-
-\begin{align*}
-    \text{if } \varphi &= \langle a \rangle \psi \quad \text{ with } a \in \Sigma \\
-    & \text{then } \textsf{expr}_6(\varphi) = \textsf{expr}_6(\psi) \\
-    \text{if } \varphi &= \bigwedge_{i \in I} \{ \psi_i \} \\
-    & \text{then } \textsf{expr}_6(\varphi) = \sup(\{\textsf{expr}_6(\psi_i)| i \in I\}) \\
-    \text{if } \psi &= \neg \varphi \\
-    & \text{then } \textsf{expr}_6(\psi) = 1 + \textsf{expr}_6(\varphi)
-\end{align*}
-\<close>
-
 primrec expr_6 :: "('a, 's)hml \<Rightarrow> enat"
   where
 expr_6_tt: \<open>expr_6 TT = 0\<close> |
@@ -272,166 +168,9 @@ expr_6_pos: \<open>expr_6 (hml_pos \<alpha> \<phi>) = expr_6 \<phi>\<close>|
 expr_6_conj: \<open>expr_6 (hml_conj I J \<Phi>) = 
 (Sup ((expr_6 \<circ> \<Phi>) ` I \<union> ((eSuc \<circ> expr_6 \<circ> \<Phi>) ` J)))\<close>
 
-text \<open>That leaves us with a definition \textsf{expr} of the expressiveness function that is easier to use.\<close>
-
 fun expr :: "('a, 's)hml \<Rightarrow> enat \<times> enat \<times> enat \<times>  enat \<times> enat \<times> enat" 
   where
 \<open>expr \<phi> = (expr_1 \<phi>, expr_2 \<phi>, expr_3 \<phi>, expr_4 \<phi>, expr_5 \<phi>, expr_6 \<phi>)\<close>
-
-text \<open>We show that \<open>direct_expr\<close> and \<open>expr\<close> are the same:\<close>
-
-
-(*<*)
-lemma expr_6_direct_expr_eq:
-  assumes "\<And>x. x \<in> \<Phi> ` I \<Longrightarrow> expr_6 x = snd (snd (snd (snd (snd (direct_expr x)))))"
-  shows "(expr_6 \<circ> \<Phi>) ` I = (snd \<circ> snd \<circ> snd \<circ> snd \<circ> snd \<circ> direct_expr \<circ> \<Phi>) ` I"
-proof -
-  have "(expr_6 \<circ> \<Phi>) ` I = (\<lambda>x. snd (snd (snd (snd (snd (direct_expr (\<Phi> x))))))) ` I"
-    by (simp add: assms)
-  also have "... = (snd \<circ> snd \<circ> snd \<circ> snd \<circ> snd \<circ> direct_expr \<circ> \<Phi>) ` I"
-    by auto
-  finally show ?thesis .
-qed
-
-lemma expr_6_eSuc_eq:
-  assumes "\<And>x. x \<in> \<Phi> ` J \<Longrightarrow> eSuc (expr_6 x) = eSuc (snd (snd (snd (snd (snd (direct_expr x))))))"
-  shows "((eSuc \<circ> expr_6 \<circ> \<Phi>) ` J) = ((eSuc \<circ> snd \<circ> snd \<circ> snd \<circ> snd \<circ> snd \<circ> direct_expr \<circ> \<Phi>) ` J)"
-proof-
-  have "((eSuc \<circ> expr_6 \<circ> \<Phi>) ` J) = (\<lambda>x. eSuc (snd (snd (snd (snd (snd (direct_expr (\<Phi> x)))))))) ` J"
-    using assms by force
-  also have "... = ((eSuc \<circ> snd \<circ> snd \<circ> snd \<circ> snd \<circ> snd \<circ> direct_expr \<circ> \<Phi>) ` J)"
-    by auto
-  finally show ?thesis.
-qed
-
-lemma expr_5_dir_eq:
-  assumes "\<forall>x \<in> \<Phi> ` (I \<union> J). expr_5 x = fst (snd (snd (snd (snd (direct_expr x)))))"
-  shows "((expr_5 \<circ> \<Phi>) ` I \<union> (expr_5 \<circ> \<Phi>) ` J) = 
-          ((fst \<circ> snd \<circ> snd \<circ> snd \<circ> snd \<circ> direct_expr \<circ> \<Phi>) ` I \<union> (fst \<circ> snd \<circ> snd \<circ> snd \<circ> snd \<circ> direct_expr \<circ> \<Phi>) ` J)"
-proof-
-  have "((expr_5 \<circ> \<Phi>) ` I \<union> (expr_5 \<circ> \<Phi>) ` J) = (\<lambda>x. fst (snd (snd (snd (snd (direct_expr (\<Phi> x))))))) ` (I \<union> J)"
-    using assms 
-    by auto
-  also have "... = (fst \<circ> snd \<circ> snd \<circ> snd \<circ> snd \<circ> direct_expr \<circ> \<Phi>) ` (I \<union> J)"
-    by auto 
-  also have "... =  ((fst \<circ> snd \<circ> snd \<circ> snd \<circ> snd \<circ> direct_expr \<circ> \<Phi>) ` I \<union> (fst \<circ> snd \<circ> snd \<circ> snd \<circ> snd \<circ> direct_expr \<circ> \<Phi>) ` J)"
-    by blast
-  finally show ?thesis.
-qed
-(*>*)
-
-lemma 
-  shows "expr \<phi> = direct_expr \<phi>"
-proof(induction \<phi>)
-  case TT
-  have "expr TT = (0, 1, 0, 0, 0, 0)" using expr.simps expr_1.simps(1) expr_2.simps(1) expr_3.simps(1) expr_4.simps(1) expr_5.simps(1) expr_6.simps(1)
-    by force
-  then show ?case using direct_expr.simps(1) 
-    by force
-next
-  case (hml_pos \<alpha> \<phi>)
-  hence IH: "(expr_1 \<phi>, expr_2 \<phi>, expr_3 \<phi>, expr_4 \<phi>, expr_5 \<phi>, expr_6 \<phi>) =
-                                (fst (direct_expr \<phi>), 
-                                fst (snd (direct_expr \<phi>)), 
-                                fst (snd (snd (direct_expr \<phi>))), 
-                                fst (snd (snd (snd (direct_expr \<phi>)))), 
-                                fst (snd (snd (snd (snd (direct_expr \<phi>))))), 
-                                snd (snd (snd (snd (snd (direct_expr \<phi>))))))"
-    by auto
-  have expr: "expr (hml_pos \<alpha> \<phi>) = (1 + (expr_1 \<phi>), expr_2 \<phi>, expr_3 \<phi>, expr_4 \<phi>, expr_5 \<phi>, expr_6 \<phi>)"
-    using expr.simps expr_1.simps expr_2.simps expr_3.simps expr_4.simps expr_5.simps expr_6.simps
-    by simp
-  have "direct_expr (hml_pos \<alpha> \<phi>) = 
-                                (1 + fst (direct_expr \<phi>), 
-                                fst (snd (direct_expr \<phi>)), 
-                                fst (snd (snd (direct_expr \<phi>))), 
-                                fst (snd (snd (snd (direct_expr \<phi>)))), 
-                                fst (snd (snd (snd (snd (direct_expr \<phi>))))), 
-                                snd (snd (snd (snd (snd (direct_expr \<phi>))))))"
-    using direct_expr.simps(2) by auto
-  then show ?case using expr IH by force
-next
-  case (hml_conj I J \<Phi>)
-  hence IH: "\<forall>\<phi> \<in> \<Phi> ` I. (expr_1 \<phi>, expr_2 \<phi>, expr_3 \<phi>, expr_4 \<phi>, expr_5 \<phi>, expr_6 \<phi>) =
-                                (fst (direct_expr \<phi>), 
-                                fst (snd (direct_expr \<phi>)), 
-                                fst (snd (snd (direct_expr \<phi>))), 
-                                fst (snd (snd (snd (direct_expr \<phi>)))), 
-                                fst (snd (snd (snd (snd (direct_expr \<phi>))))), 
-                                snd (snd (snd (snd (snd (direct_expr \<phi>))))))"
-        "\<forall>\<phi> \<in> \<Phi> ` J. (expr_1 \<phi>, expr_2 \<phi>, expr_3 \<phi>, expr_4 \<phi>, expr_5 \<phi>, expr_6 \<phi>) =
-                                (fst (direct_expr \<phi>), 
-                                fst (snd (direct_expr \<phi>)), 
-                                fst (snd (snd (direct_expr \<phi>))), 
-                                fst (snd (snd (snd (direct_expr \<phi>)))), 
-                                fst (snd (snd (snd (snd (direct_expr \<phi>))))), 
-                                snd (snd (snd (snd (snd (direct_expr \<phi>))))))"
-    by simp+
-  hence e1: "Sup ((expr_1 \<circ> \<Phi>) ` I \<union> (expr_1 \<circ> \<Phi>) ` J) = Sup ((fst \<circ> direct_expr \<circ> \<Phi>) ` I \<union> (fst \<circ> direct_expr \<circ> \<Phi>) ` J)"
-    by (smt (verit, best) Pair_inject comp_apply image_cong image_eqI)
-  have e2: "1 + Sup ((expr_2 \<circ> \<Phi>) ` I \<union> (expr_2 \<circ> \<Phi>) ` J) = 1 + Sup ((fst \<circ> snd \<circ> direct_expr \<circ> \<Phi>) ` I \<union> (fst \<circ> snd \<circ> direct_expr \<circ> \<Phi>) ` J)"
-    using IH Sup_le_iff 
-    by (smt (verit) Pair_inject comp_apply image_cong image_eqI)
-  have e3: "(Sup ((expr_1 \<circ> \<Phi>) ` I \<union> (expr_3 \<circ> \<Phi>) ` I \<union> (expr_3 \<circ> \<Phi>) ` J)) =
-        (Sup ((fst \<circ> direct_expr \<circ> \<Phi>) ` I \<union> (fst \<circ> snd \<circ> snd \<circ> direct_expr \<circ> \<Phi>) ` I \<union> (fst \<circ> snd \<circ> snd \<circ> direct_expr \<circ> \<Phi>) ` J))"
-    using IH Sup_le_iff 
-    by (smt (verit, ccfv_SIG) Pair_inject comp_apply image_comp image_cong)
-  have e4: "Sup ((expr_1 ` (pos_r (\<Phi> ` I)))  \<union> (expr_4 \<circ> \<Phi>) ` I \<union> (expr_4 \<circ> \<Phi>) ` J) =
-        (Sup (((fst \<circ> direct_expr) ` (pos_r (\<Phi> ` I)))  \<union> (fst \<circ> snd \<circ> snd \<circ> snd \<circ> direct_expr \<circ> \<Phi>) ` I \<union> (fst \<circ> snd \<circ> snd \<circ> snd \<circ> direct_expr \<circ> \<Phi>) ` J))"
-  proof-
-    have sup_pos_r: "\<forall>x \<in> pos_r (\<Phi> ` I). expr_1 x = (fst \<circ> direct_expr) x"
-      using IH 
-      by (metis (no_types, lifting) Diff_iff Pair_inject comp_apply pos_r.simps)
-    hence "Sup (expr_1 ` pos_r (\<Phi> ` I)) = Sup ((fst \<circ> direct_expr) ` pos_r (\<Phi> ` I))"
-      by (meson SUP_cong)
-    have "\<forall>x \<in> \<Phi> ` (I \<union> J). expr_4 x = fst (snd (snd (snd (direct_expr x))))"
-      using IH
-      by blast+
-    hence "Sup ((expr_4 \<circ> \<Phi>) ` I \<union> (expr_4 \<circ> \<Phi>) ` J) = 
-          Sup ((fst \<circ> snd \<circ> snd \<circ> snd \<circ> direct_expr \<circ> \<Phi>) ` I \<union>
-          (fst \<circ> snd \<circ> snd \<circ> snd \<circ> direct_expr \<circ> \<Phi>) ` J)"
-      using SUP_cong by auto
-    then show ?thesis using sup_pos_r 
-      by (metis (no_types, lifting) Sup_union_distrib image_cong inf_sup_aci(6))
-  qed
-  have e5: "(Sup ((expr_5 \<circ> \<Phi>) ` I \<union> (expr_5 \<circ> \<Phi>) ` J \<union> (expr_1 \<circ> \<Phi>) ` J)) =
-  (Sup ((fst \<circ> snd \<circ> snd \<circ> snd \<circ> snd \<circ> direct_expr \<circ> \<Phi>) ` I \<union> (fst \<circ> snd \<circ> snd \<circ> snd \<circ> snd \<circ> direct_expr \<circ> \<Phi>) ` J \<union> (fst \<circ> direct_expr \<circ> \<Phi>) ` J))"
-    using IH
-  proof-
-    have fa_e5: "\<forall>x \<in> \<Phi> ` (I \<union> J). expr_5 x = fst (snd (snd (snd (snd (direct_expr x)))))"
-          "\<forall>x \<in> \<Phi> ` J. expr_1 x = fst (direct_expr x)"
-      using IH 
-      by blast+
-    hence "Sup ((expr_1 \<circ> \<Phi>) ` J )= Sup ((fst \<circ> direct_expr \<circ> \<Phi>) ` J)" 
-      by fastforce
-    have "Sup ((expr_5 \<circ> \<Phi>) ` I \<union> (expr_5 \<circ> \<Phi>) ` J) = 
-          Sup ((fst \<circ> snd \<circ> snd \<circ> snd \<circ> snd \<circ> direct_expr \<circ> \<Phi>) ` I \<union> (fst \<circ> snd \<circ> snd \<circ> snd \<circ> snd \<circ> direct_expr \<circ> \<Phi>) ` J)"
-      using expr_5_dir_eq fa_e5 by force
-    then show ?thesis 
-      using \<open>Sup ((expr_1 \<circ> \<Phi>) ` J )= Sup ((fst \<circ> direct_expr \<circ> \<Phi>) ` J)\<close> 
-      by (simp add: Sup_union_distrib)
-  qed
-
-  have e6: "(Sup ((expr_6 \<circ> \<Phi>) ` I \<union> ((eSuc \<circ> expr_6 \<circ> \<Phi>) ` J))) =
-        (Sup ((snd \<circ> snd \<circ> snd \<circ> snd \<circ> snd \<circ> direct_expr \<circ> \<Phi>) ` I \<union> ((eSuc \<circ> snd \<circ> snd \<circ> snd \<circ> snd \<circ> snd \<circ> direct_expr \<circ> \<Phi>) ` J)))"
-  proof-
-    have "\<forall>x \<in> \<Phi> ` I. expr_6 x = snd (snd (snd (snd (snd (direct_expr x)))))"
-          "\<forall>x \<in> \<Phi> ` J. expr_6 x = snd (snd (snd (snd (snd (direct_expr x)))))"
-      using IH by blast+
-    from this(1) have "((expr_6 \<circ> \<Phi>) ` I) = ((snd \<circ> snd \<circ> snd \<circ> snd \<circ> snd \<circ> direct_expr \<circ> \<Phi>) ` I)"
-      using expr_6_direct_expr_eq by force
-    hence "Sup ((expr_6 \<circ> \<Phi>) ` I) = Sup ((snd \<circ> snd \<circ> snd \<circ> snd \<circ> snd \<circ> direct_expr \<circ> \<Phi>) ` I)"
-      by presburger 
-    have "\<forall>x \<in> \<Phi> ` J. eSuc (expr_6 x) = eSuc (snd (snd (snd (snd (snd (direct_expr x))))))"
-      using \<open>\<forall>x \<in> \<Phi> ` J. expr_6 x = snd (snd (snd (snd (snd (direct_expr x)))))\<close> by simp
-    hence "Sup ((eSuc \<circ> expr_6 \<circ> \<Phi>) ` J) = Sup ((eSuc \<circ> snd \<circ> snd \<circ> snd \<circ> snd \<circ> snd \<circ> direct_expr \<circ> \<Phi>) ` J)"
-      using expr_6_eSuc_eq by auto
-    then show ?thesis using \<open>Sup ((expr_6 \<circ> \<Phi>) ` I) = Sup ((snd \<circ> snd \<circ> snd \<circ> snd \<circ> snd \<circ> direct_expr \<circ> \<Phi>) ` I)\<close>
-      by (simp add: Sup_union_distrib)
-  qed
-
-  then show ?case using e1 e2 e3 e4 e5 e6 by simp
-qed
 
 text \<open>Prices are compared component wise, i.e., $(e_1, \ldots e_6) \leq (f_1 \ldots f_6)$ iff $e_i \leq f_i$ for each $i$.\<close>
 
@@ -451,7 +190,359 @@ definition e_sup :: "(enat \<times> enat \<times> enat \<times> enat \<times> en
 (Sup ((snd \<circ> snd \<circ> snd \<circ> snd \<circ> snd) ` S)))"
 (*>*)
 
-text \<open>\textbf{Proposition} The expressiveness function is monotonic.\<close>
+text \<open>\begin{figure}[t]
+    \centering
+\begin{multicols}{2}
+
+\columnbreak
+\begin{tikzpicture}[-, >=stealth, node distance=1.2cm, every node/.style={minimum size=0.3cm}]
+    \node (p1) {$\langle a \rangle$};
+    \node (p2) [below of=p1] {$\bigwedge$};
+    \node (p3) [below left=of p2] {$\langle b \rangle$};
+    \node (p4) [below right=of p2] {$\langle a \rangle$};
+    \node (p5) [below of=p3] {$\bigwedge$};
+    \node (p6) [below of=p4] {$\bigwedge$};
+    \node (p7) [below left of=p6] {$\lnot$};
+    \node (p8) [below right of=p6] {$\lnot$};
+    \node (p9) [below of=p7] {$\langle a \rangle$};
+    \node (p10) [below of=p9] {$\langle c \rangle$};
+    \node (p11) [below of=p10] {$\bigwedge$};
+    \node (p12) [below of=p8] {$\langle b \rangle$};
+    \node (p13) [below of=p12] {$\bigwedge$};
+
+    \path[-] (p1) edge (p2);
+    \path[-] (p2) edge (p3);
+    \path[-] (p2) edge (p4);
+    \path[-] (p3) edge (p5);
+    \path[-] (p4) edge (p6);
+    \path[-] (p6) edge (p7);
+    \path[-] (p6) edge (p8);
+    \path[-] (p7) edge (p9);
+    \path[-] (p9) edge (p10);
+    \path[-] (p10) edge (p11);
+    \path[-] (p8) edge (p12);
+    \path[-] (p12) edge (p13);
+
+  \node[circle, draw=red, fill=red, inner sep=0.3pt, minimum size=3pt] (v11) at (4,0) {};
+  \node[circle, draw=red, fill=red, inner sep=0.3pt, minimum size=3pt] (v12) at (4,-2.67) {};
+  \node[circle, draw=red, fill=red, inner sep=0.3pt, minimum size=3pt] (v12) at (4,-6) {};
+  \node[circle, draw=red, fill=red, inner sep=0.3pt, minimum size=3pt] (v13) at (4,-7.2) {};
+  \node (v14) at (4,-8.7) {};
+  \node (v21) at (5,0.2) {};
+  \node[circle, draw=orange, fill=orange, inner sep=0.3pt, minimum size=3pt] (v22) at (5,-1.2) {};
+  \node[circle, draw=orange, fill=orange, inner sep=0.3pt, minimum size=3pt] (v23) at (5,-3.8) {};
+  \node[circle, draw=orange, fill=orange, inner sep=0.3pt, minimum size=3pt] (v24) at (5,-7.2) {};
+  \node (v25) at (5,-8.7) {};
+  \node (v31) at (6,0.2) {};
+  \node[circle, draw=myyellow, fill=myyellow, inner sep=0.3pt, minimum size=3pt] (v32) at (6,-2.67) {};
+  \node[circle, draw=myyellow, fill=myyellow, inner sep=0.3pt, minimum size=3pt] (v32) at (6,-6) {};
+  \node[circle, draw=myyellow, fill=myyellow, inner sep=0.3pt, minimum size=3pt] (v33) at (6,-7.2) {};
+  \node (v34) at (6,-8.7) {};
+  \node (v41) at (7,0.2) {};
+  \node[circle, draw=green, fill=green, inner sep=0.3pt, minimum size=3pt] (v42) at (7,-2.67) {};
+  \node (v43) at (7,-8.7) {};
+  \node (v51) at (8,0.2) {};
+  \node[circle, draw=cyan, fill=cyan, inner sep=0.3pt, minimum size=3pt] (v52) at (8,-6) {};
+  \node[circle, draw=cyan, fill=cyan, inner sep=0.3pt, minimum size=3pt] (v53) at (8,-7.2) {};
+  \node (v54) at (8,-8.7) {};
+  \node (v61) at (9,0.2) {};
+  \node[circle, draw=violet, fill=violet, inner sep=0.3pt, minimum size=3pt] (v62) at (9,-5.2) {};
+  \node (v63) at (9,-8.7) {};
+
+  \path[-, red] (v11) edge (v14);
+  \path[-, orange] (v21) edge (v25);
+  \path[-, myyellow] (v31) edge (v34);
+  \path[-, green] (v41) edge (v43);
+  \path[-, cyan] (v51) edge (v54);
+  \path[-, violet] (v61) edge (v63);
+
+
+\end{tikzpicture}
+\end{multicols}
+\caption{Pricing of formula $\langle a \rangle \bigwedge \{\langle b \rangle, \langle a \rangle \bigwedge \{\lnot \langle a \rangle \langle c \rangle, \lnot \langle b \rangle\}\}$}
+    \label{fig:2_3}
+\end{figure}\<close>
+
+lemma example_2_3:
+  fixes s and t and a and b and c
+  assumes "s \<noteq> t"
+  defines \<phi>: "(\<phi>::('a, 's)hml) \<equiv> 
+  (hml_pos a 
+    (hml_conj {s, t} {}
+      (\<lambda>i. (if i = s 
+            then (hml_pos b TT) 
+            else 
+              (if i = t  
+               then (hml_pos a 
+                      (hml_conj {} {s, t} 
+                        (\<lambda>j. (if j = s 
+                              then (hml_pos a 
+                                     (hml_pos c TT)) 
+                              else 
+                                (if j = t 
+                                 then (hml_pos b TT) 
+                                 else undefined)))))
+               else undefined)))))"
+
+shows 
+  "expr_1 \<phi> = 4"
+  "expr_2 \<phi> = 3"
+  "expr_3 \<phi> = 3"
+  "expr_4 \<phi> = 1"
+  "expr_5 \<phi> = 2"
+  "expr_6 \<phi> = 1"
+  proof- 
+    have "expr_1 (hml_pos a (hml_pos c TT)) = 2" "expr_1 (hml_pos b TT) = 1"
+      by simp+
+    hence "Sup ((expr_1 \<circ> (\<lambda>j. if j = s then hml_pos a (hml_pos c TT)
+                                    else if j = t then hml_pos b TT else undefined)) ` {s, t}) = 2"
+      by (smt (verit, best) SUP_insert Sup_empty assms(1) ile_eSuc image_is_empty o_apply one_add_one plus_1_eSuc(1) sup.orderE sup_bot.right_neutral)
+    hence "expr_1 (hml_conj {} {s, t}
+                              (\<lambda>j. if j = s then hml_pos a (hml_pos c TT)
+                                    else if j = t then hml_pos b TT else undefined)) = 2"
+      using expr_1_conj 
+      by auto
+    hence 1: "expr_1 (hml_pos a
+                            (hml_conj {} {s, t}
+                              (\<lambda>j. if j = s then hml_pos a (hml_pos c TT)
+                                    else if j = t then hml_pos b TT else undefined))) = 3"
+      and 2: "expr_1 ( hml_pos b TT) = 1"
+      by force+
+    hence "Sup ((expr_1 \<circ> (\<lambda>i. if i = s then hml_pos b TT
+                 else if i = t
+                      then hml_pos a
+                            (hml_conj {} {s, t}
+                              (\<lambda>j. if j = s then hml_pos a (hml_pos c TT)
+                                    else if j = t then hml_pos b TT else undefined))
+                      else undefined)) ` {s, t}) = 3"
+      using "1" SUP_insert Sup_empty assms(1) image_is_empty o_apply one_le_numeral sup.orderE sup_bot.right_neutral sup_commute
+      by (smt (verit, del_insts) ile_eSuc numeral_Bit1 numeral_One one_add_one one_plus_numeral_commute plus_1_eSuc(1))
+    
+    hence "expr_1 (hml_conj {s, t} {}
+           (\<lambda>i. if i = s then hml_pos b TT
+                 else if i = t
+                      then hml_pos a
+                            (hml_conj {} {s, t}
+                              (\<lambda>j. if j = s then hml_pos a (hml_pos c TT)
+                                    else if j = t then hml_pos b TT else undefined))
+                      else undefined)) = 3" 
+      by simp
+    thus e1: "expr_1 \<phi> = 4"  
+      unfolding \<phi> 
+      by fastforce
+
+    show e2: "expr_2 \<phi> = 3" 
+      unfolding \<phi>  
+      by (smt (z3) "1" "2" SUP_empty SUP_insert Un_insert_right \<open>Sup ((expr_1 \<circ> (\<lambda>j. if j = s then hml_pos a (hml_pos c TT) else if j = t then hml_pos b TT else undefined)) ` {s, t}) = 2\<close> \<open>expr_1 (hml_conj {} {s, t} (\<lambda>j. if j = s then hml_pos a (hml_pos c TT) else if j = t then hml_pos b TT else undefined)) = 2\<close> assms(1) comp_def expr_1_pos expr_2_conj expr_2_pos expr_2_tt image_Un insert_is_Un numeral_One one_le_numeral sup.order_iff sup_bot_right)
+
+    show e3: "expr_3 \<phi> = 3"
+    proof-
+      have e3_1: "expr_3 (hml_conj {} {s, t} 
+                        (\<lambda>j. (if j = s 
+                              then (hml_pos a 
+                                     (hml_pos c TT)) 
+                              else 
+                                (if j = t 
+                                 then (hml_pos b TT) 
+                                 else undefined)))) = 0"
+        by simp
+      hence e1_1: "(Sup ((expr_1 \<circ> (\<lambda>i. (if i = s 
+            then (hml_pos b TT) 
+            else 
+              (if i = t  
+               then (hml_pos a 
+                      (hml_conj {} {s, t} 
+                        (\<lambda>j. (if j = s 
+                              then (hml_pos a 
+                                     (hml_pos c TT)) 
+                              else 
+                                (if j = t 
+                                 then (hml_pos b TT) 
+                                 else undefined)))))
+               else undefined)))) ` {s, t})) = 3"
+        using \<open>Sup ((expr_1 \<circ> (\<lambda>i. if i = s then hml_pos b TT else if i = t then hml_pos a (hml_conj {} {s, t} (\<lambda>j. if j = s then hml_pos a (hml_pos c TT) else if j = t then hml_pos b TT else undefined)) else undefined)) ` {s, t}) = 3\<close> by blast
+      have "(Sup ((expr_3 \<circ> (\<lambda>i. (if i = s 
+            then (hml_pos b TT) 
+            else 
+              (if i = t  
+               then (hml_pos a 
+                      (hml_conj {} {s, t} 
+                        (\<lambda>j. (if j = s 
+                              then (hml_pos a 
+                                     (hml_pos c TT)) 
+                              else 
+                                (if j = t 
+                                 then (hml_pos b TT) 
+                                 else undefined)))))
+               else undefined)))) ` {s, t})) = 0"
+        
+        by simp
+      hence "expr_3  
+    (hml_conj {s, t} {}
+      (\<lambda>i. (if i = s 
+            then (hml_pos b TT) 
+            else 
+              (if i = t  
+               then (hml_pos a 
+                      (hml_conj {} {s, t} 
+                        (\<lambda>j. (if j = s 
+                              then (hml_pos a 
+                                     (hml_pos c TT)) 
+                              else 
+                                (if j = t 
+                                 then (hml_pos b TT) 
+                                 else undefined)))))
+               else undefined)))) = 3"
+        using e1_1
+        by (smt (verit, best) Sup_union_distrib bot_enat_def expr_3_conj image_empty sup_bot.right_neutral)
+      thus ?thesis
+        unfolding \<phi> 
+        by fastforce
+    qed
+
+    show e5: "expr_5 \<phi> = 2"
+    proof-
+      have "expr_5 (hml_pos b TT) = 0"
+        by fastforce
+      have "expr_5 (hml_conj {} {s, t} 
+                        (\<lambda>j. (if j = s 
+                              then (hml_pos a 
+                                     (hml_pos c TT)) 
+                              else 
+                                (if j = t 
+                                 then (hml_pos b TT) 
+                                 else undefined)))) = 2"
+        using \<open>Sup ((expr_1 \<circ> (\<lambda>j. if j = s then hml_pos a (hml_pos c TT) else if j = t then hml_pos b TT else undefined)) ` {s, t}) = 2\<close> bot_enat_def by auto
+
+      hence "expr_5 (hml_conj {s, t} {}
+      (\<lambda>i. (if i = s 
+            then (hml_pos b TT) 
+            else 
+              (if i = t  
+               then (hml_pos a 
+                      (hml_conj {} {s, t} 
+                        (\<lambda>j. (if j = s 
+                              then (hml_pos a 
+                                     (hml_pos c TT)) 
+                              else 
+                                (if j = t 
+                                 then (hml_pos b TT) 
+                                 else undefined)))))
+               else undefined)))) = 2"
+        using \<open>expr_5 (hml_pos b TT) = 0\<close> image_insert SUP_insert Sup_union_distrib Un_insert_left Un_insert_right \<open>Sup ((expr_1 \<circ> (\<lambda>j. if j = s then hml_pos a (hml_pos c TT) else if j = t then hml_pos b TT else undefined)) ` {s, t}) = 2\<close> assms(1) comp_apply expr_5_conj expr_5_pos image_Un image_empty insert_absorb insert_iff insert_is_Un
+        
+      proof -
+        assume "Sup ((expr_1 \<circ> (\<lambda>j. if j = s then hml_pos a (hml_pos c TT) else if j = t then hml_pos b TT else undefined)) ` {s, t}) = 2"
+        have f1: "(expr_5 \<circ> (\<lambda>sa. if sa = s then hml_pos a (hml_pos c (TT::('a, 's) hml)) else if sa = t then hml_pos b TT else undefined)) ` {} \<union> (expr_5 \<circ> (\<lambda>sa. if sa = s then hml_pos a (hml_pos c (TT::('a, 's) hml)) else if sa = t then hml_pos b TT else undefined)) ` {s, t} \<union> (expr_1 \<circ> (\<lambda>sa. if sa = s then hml_pos a (hml_pos c (TT::('a, 's) hml)) else if sa = t then hml_pos b TT else undefined)) ` {s, t} = (expr_5 \<circ> (\<lambda>sa. if sa = s then hml_pos a (hml_pos c (TT::('a, 's) hml)) else if sa = t then hml_pos b TT else undefined)) ` {} \<union> (expr_5 \<circ> (\<lambda>sa. if sa = s then hml_pos a (hml_pos c (TT::('a, 's) hml)) else if sa = t then hml_pos b TT else undefined)) ` {t, s} \<union> insert ((expr_1 \<circ> (\<lambda>sa. if sa = s then hml_pos a (hml_pos c (TT::('a, 's) hml)) else if sa = t then hml_pos b TT else undefined)) t) ((expr_1 \<circ> (\<lambda>sa. if sa = s then hml_pos a (hml_pos c (TT::('a, 's) hml)) else if sa = t then hml_pos b TT else undefined)) ` {s})"
+          by (simp add: insert_commute)
+        have f2: "expr_5 (TT::('a, 's) hml) = expr_5 (if t = s then hml_pos a (hml_pos c (TT::('a, 's) hml)) else if t = t then hml_pos b TT else undefined)"
+          by auto
+        have f3: "insert (expr_5 (if t = s then hml_pos a (hml_pos c (TT::('a, 's) hml)) else if t = t then hml_pos b TT else undefined)) (insert ((expr_5 \<circ> (\<lambda>sa. if sa = s then hml_pos a (hml_pos c (TT::('a, 's) hml)) else if sa = t then hml_pos b TT else undefined)) s) ((expr_5 \<circ> (\<lambda>sa. if sa = s then hml_pos a (hml_pos c (TT::('a, 's) hml)) else if sa = t then hml_pos b TT else undefined)) ` {})) = (expr_5 \<circ> (\<lambda>sa. if sa = s then hml_pos a (hml_pos c (TT::('a, 's) hml)) else if sa = t then hml_pos b TT else undefined)) ` {} \<union> (expr_5 \<circ> (\<lambda>sa. if sa = s then hml_pos a (hml_pos c (TT::('a, 's) hml)) else if sa = t then hml_pos b TT else undefined)) ` {t, s}"
+          by auto
+        have "expr_5 (hml_conj {s, t} {} (\<lambda>sa. if sa = s then hml_pos b TT else if sa = t then hml_pos a (hml_conj {} {s, t} (\<lambda>sa. if sa = s then hml_pos a (hml_pos c TT) else if sa = t then hml_pos b TT else undefined)) else undefined)) = Sup (insert ((expr_5 \<circ> (\<lambda>sa. if sa = s then hml_pos a (hml_pos c (TT::('a, 's) hml)) else if sa = t then hml_pos b TT else undefined)) s) ((expr_5 \<circ> (\<lambda>sa. if sa = s then hml_pos a (hml_pos c (TT::('a, 's) hml)) else if sa = t then hml_pos b TT else undefined)) ` {}) \<union> insert ((expr_1 \<circ> (\<lambda>sa. if sa = s then hml_pos a (hml_pos c (TT::('a, 's) hml)) else if sa = t then hml_pos b TT else undefined)) t) ((expr_1 \<circ> (\<lambda>sa. if sa = s then hml_pos a (hml_pos c (TT::('a, 's) hml)) else if sa = t then hml_pos b TT else undefined)) ` {s}) \<union> insert ((expr_5 \<circ> (\<lambda>sa. if sa = s then hml_pos a (hml_pos c (TT::('a, 's) hml)) else if sa = t then hml_pos b TT else undefined)) s) ((expr_5 \<circ> (\<lambda>sa. if sa = s then hml_pos a (hml_pos c (TT::('a, 's) hml)) else if sa = t then hml_pos b TT else undefined)) ` {}))"
+          using f1 \<open>s \<noteq> t\<close> by auto
+        then show ?thesis
+          using f3 f2 by (smt (z3) \<open>\<And>a A. insert a A = {a} \<union> A\<close> \<open>\<And>a C B. insert a B \<union> C = insert a (B \<union> C)\<close> \<open>\<And>f B A. f ` (A \<union> B) = f ` A \<union> f ` B\<close> \<open>\<And>f a B. f ` insert a B = insert (f a) (f ` B)\<close> \<open>\<And>x g f. (f \<circ> g) x = f (g x)\<close> \<open>expr_5 (hml_conj {} {s, t} (\<lambda>j. if j = s then hml_pos a (hml_pos c TT) else if j = t then hml_pos b TT else undefined)) = 2\<close> empty_is_image expr_5_conj expr_5_pos insert_commute)
+      qed
+      thus ?thesis
+        unfolding \<phi>
+        by force
+    qed
+
+    show e6: "expr_6 \<phi> = 1"
+    proof-
+      have e6_1: "Sup ((expr_6 \<circ> (\<lambda>j. if j = s then hml_pos a (hml_pos c TT)
+                                  else if j = t then hml_pos b TT else undefined)) ` {}) = 0"
+        using bot_enat_def by force 
+      have "Sup (((expr_6 \<circ> (\<lambda>j. if j = s then hml_pos a (hml_pos c TT)
+                                  else if j = t then hml_pos b TT else undefined)) ` {s, t})) = 0"
+        by simp
+      hence e6_2: "Sup (((eSuc \<circ> expr_6 \<circ> (\<lambda>j. if j = s then hml_pos a (hml_pos c TT)
+                                  else if j = t then hml_pos b TT else undefined)) ` {s, t})) = 1"
+        using eSuc_def 
+        by (simp add: one_eSuc)
+      thus "expr_6 \<phi> = 1"
+        unfolding \<phi>
+        using e6_1 
+        by (smt (z3) SUP_insert assms(1) ccSUP_empty comp_def empty_is_image expr_6.simps(1) expr_6.simps(2) expr_6_conj sup_bot.left_neutral sup_bot_right)
+    qed
+
+      have "(expr_1 ` (pos_r ((\<lambda>j. if j = s then hml_pos a (hml_pos c TT)
+                                    else if j = t then hml_pos b TT else undefined) ` {}))) = {}"
+  "((expr_4 \<circ> (\<lambda>j. if j = s then hml_pos a (hml_pos c TT)
+                                    else if j = t then hml_pos b TT else undefined)) ` {}) = {}"
+      by auto
+    hence "Sup (expr_1 ` (pos_r ((\<lambda>j. if j = s then hml_pos a (hml_pos c TT)
+                                    else if j = t then hml_pos b TT else undefined) ` {}))) = 0"
+          "Sup((expr_4 \<circ> (\<lambda>j. if j = s then hml_pos a (hml_pos c TT)
+                                    else if j = t then hml_pos b TT else undefined)) ` {}) = 0"
+          "Sup((expr_4 \<circ> (\<lambda>j. if j = s then hml_pos a (hml_pos c TT)
+                                    else if j = t then hml_pos b TT else undefined)) ` {s, t}) = 0"
+      using bot_enat_def by fastforce+
+    hence "Sup ((expr_1 ` (pos_r ((\<lambda>j. if j = s then hml_pos a (hml_pos c TT)
+                                    else if j = t then hml_pos b TT else undefined) ` {})))  \<union> (expr_4 \<circ> (\<lambda>j. if j = s then hml_pos a (hml_pos c TT)
+                                    else if j = t then hml_pos b TT else undefined)) ` {} \<union> (expr_4 \<circ> (\<lambda>j. if j = s then hml_pos a (hml_pos c TT)
+                                    else if j = t then hml_pos b TT else undefined)) ` {s, t}) = 0" by simp
+    hence "expr_4 (hml_pos a
+                            (hml_conj {} {s, t}
+                              (\<lambda>j. if j = s then hml_pos a (hml_pos c TT)
+                                    else if j = t then hml_pos b TT else undefined))) = 0"
+      by simp
+    have "(pos_r ((\<lambda>i. if i = s then hml_pos b TT
+                 else if i = t
+                      then hml_pos a
+                            (hml_conj {} {s, t}
+                              (\<lambda>j. if j = s then hml_pos a (hml_pos c TT)
+                                    else if j = t then hml_pos b TT else undefined))
+                      else undefined) ` {s, t})) = 
+                          {hml_pos b TT}"
+    proof-
+      define xs where "xs \<equiv> ((\<lambda>i. if i = s then hml_pos b TT
+                 else if i = t
+                      then hml_pos a
+                            (hml_conj {} {s, t}
+                              (\<lambda>j. if j = s then hml_pos a (hml_pos c TT)
+                                    else if j = t then hml_pos b TT else undefined))
+                      else undefined) ` {s, t})"
+      have "(Sup (expr_1 ` xs)) = 3" 
+        unfolding xs_def
+        by (metis Sup.SUP_image \<open>Sup ((expr_1 \<circ> (\<lambda>i. if i = s then hml_pos b TT else if i = t then hml_pos a (hml_conj {} {s, t} (\<lambda>j. if j = s then hml_pos a (hml_pos c TT) else if j = t then hml_pos b TT else undefined)) else undefined)) ` {s, t}) = 3\<close>)
+      hence "{\<psi> | \<psi>. \<psi> \<in> xs \<and> (expr_1 \<psi> = (Sup (expr_1 ` xs)))} =
+              {(hml_pos a
+                            (hml_conj {} {s, t}
+                              (\<lambda>j. if j = s then hml_pos a (hml_pos c TT)
+                                    else if j = t then hml_pos b TT else undefined)))}"
+        using 1 2 assms(1) xs_def by force
+      hence "(SOME \<psi>. \<psi> \<in> xs \<and> expr_1 \<psi> = (Sup (expr_1 ` xs))) =
+              (hml_pos a
+                            (hml_conj {} {s, t}
+                              (\<lambda>j. if j = s then hml_pos a (hml_pos c TT)
+                                    else if j = t then hml_pos b TT else undefined)))"
+        unfolding xs_def
+        using pos_r.simps 2 1 assms(1)
+        by (smt (verit, ccfv_threshold) mem_Collect_eq singleton_iff someI_ex)
+      then show ?thesis 
+        unfolding xs_def
+        using pos_r.simps assms(1) by auto
+    qed
+    hence "Sup ((expr_1 ` (pos_r ((\<lambda>i. if i = s then hml_pos b TT
+                 else if i = t
+                      then hml_pos a
+                            (hml_conj {} {s, t}
+                              (\<lambda>j. if j = s then hml_pos a (hml_pos c TT)
+                                    else if j = t then hml_pos b TT else undefined))
+                      else undefined) ` {s, t})))) = 1" 
+      using "1" by auto
+    then show "expr_4 \<phi> = 1" 
+      unfolding \<phi>
+      by (smt (verit, del_insts) SUP_insert Sup_union_distrib \<open>expr_4 (hml_pos a (hml_conj {} {s, t} (\<lambda>j. if j = s then hml_pos a (hml_pos c TT) else if j = t then hml_pos b TT else undefined))) = 0\<close> bot_enat_def ccSUP_empty comp_apply expr_4_conj expr_4_pos expr_4_tt sup_bot.right_neutral)
+  qed
+
+  text \<open>\textit{Example 2}: This example illustrates how the prices of a formula are calculated. In Figure \ref{fig:2_3}, you can see the pricing process for the formula $\langle a \rangle \bigwedge \{\langle b \rangle, \langle a \rangle \bigwedge \{\lnot \langle a \rangle \langle c \rangle, \lnot \langle b \rangle\}\}$. Each line to the right of the syntax tree represents the price of a specific dimension. The circles of each line represent an increase in the price of that dimension. The colors of these lines correspond to those defined in (ref definition 2.3.1) and indicate the dimension they represent. Note the finishing empty conjunction, which increases the conjunction depth by one.
+We can use the function to calculate the prices of the formulas in Example 1. The price of $\varphi_1 :=\langle a \rangle\bigwedge\{\lnot\langle c \rangle\}$ is $expr(\varphi_1) = (2, 2, 0, 0, 1, 1)$. For $\varphi_2 := \bigwedge\{\lnot\langle a \rangle\bigwedge\{\lnot\langle c \rangle\}\}$, $expr(\varphi_2) = (2, 3, 0, 0, 2, 2)$.
+\<close>
+text \<open>\textbf{Proposition} The expressiveness function is monotonic. Specifically, for any formula $\langle\alpha\rangle\varphi$, is the expressiveness of the subformula $\varphi$ less than or equal to the expressiveness of $\langle\alpha\rangle\varphi$.
+Similarly, for any conjunctive formula $\bigwedge_{i\in I}\psi_i$, the expressiveness of every conjunct $\psi_i$ is less than or equal to the expressiveness of $\bigwedge_{i\in I}\psi_i$.\<close>
 
 lemma mon_pos:
   fixes n1 and n2 and n3 and n4::enat and n5 and n6 and \<alpha>
@@ -547,6 +638,8 @@ expr.simps less_eq_t.simps
 expr.simps less_eq_t.simps
     by (simp add: Sup_le_iff)
 qed
+
+
 
 (*<*)
 end
