Alternative_price_function.thy
@@ -1,0 +1,288 @@
+(*<*)
+theory Alternative_price_function
+imports
+  formula_prices_list
+begin
+(*>*)
+chapter \<open>Alternative price function\<close>
+text \<open>\label{chap:alternative_price_function}\<close>
+
+text \<open>Den Rest in den Appendix:\<close>
+
+text \<open>\textit{
+The expressiveness price $\textsf{expr} : \text{HML}[\Sigma] \rightarrow (\mathbb{N \cup \infty})^6$ of a formula interpreted as $6 \times 1$-dimensional vectors is defined recursively by:}
+
+\begin{minipage}{0.45\textwidth}
+\[
+\text{expr}(\langle a \rangle \varphi) :=
+\begin{pmatrix}
+1 + \text{expr}_1(\varphi) \\
+\text{expr}_2(\varphi) \\
+\text{expr}_3(\varphi) \\
+\text{expr}_4(\varphi) \\
+\text{expr}_5(\varphi) \\
+\text{expr}_6(\varphi) \\
+\end{pmatrix}
+\]
+\end{minipage}
+\hfill
+\begin{minipage}{0.45\textwidth}
+\[
+\text{expr}(\neg \varphi) := 
+\begin{pmatrix}
+\text{expr}_1(\varphi) \\
+\text{expr}_2(\varphi) \\
+\text{expr}_3(\varphi) \\
+\text{expr}_4(\varphi) \\
+\text{expr}_5(\varphi) \\
+1 + \text{expr}_6(\varphi) \\
+\end{pmatrix}
+\]
+\end{minipage}
+
+\[
+\text{expr}\left( \bigwedge_{i \in I} \psi_i \right) := \sup(\{
+\begin{pmatrix}
+0 \\
+1 + \sup_{i \in I} \text{expr}_2(\psi_i) \\
+\sup_{i \in \text{Pos}} \text{expr}_1(\psi_i) \\
+\sup_{i \in \text{Pos} \backslash \mathcal{R}} \text{expr}_1(\psi_i) \\
+\sup_{i \in \text{Neg}} \text{expr}_1(\psi_i) \\
+0 \\
+\end{pmatrix} \} \cup \{\textsf{expr}(\psi_i) | i \in I\} 
+\]
+
+Remark: The only deviation from \cite{bisping2023process} (Definition 5) is, that we include infinity in the range of the function since we allow for infinite branching conjunctions.
+
+It turned out that it was easier to also define the price for every dimension i as a seperate function $\textsf{expr} : \text{HML}[\Sigma] \rightarrow (\mathbb{N \cup \infty})$.\<close>
+
+text \<open>Our Isabelle definition of HML makes it very easy to derive the sets Pos and Neg, by \<open>\<Phi> ` I\<close> and \<open>\<Phi> ` J\<close> respectively.\<close>
+text \<open>Vlt als erstes: modaltiefe als beispiel für observation expressiveness von formel, mit isabelle definition,
+dann pos\_r definition,
+direct\_expr definition,
+einzelne dimensionen,
+lemma direct\_expr = expr...\<close>
+
+text \<open>Now we can directly define the expressiveness function as \<open>direct_expr\<close>.\<close>
+
+function direct_expr :: "('a, 's)hml \<Rightarrow> enat \<times> enat \<times> enat \<times> enat \<times> enat \<times> enat" where
+  "direct_expr TT = (0, 1, 0, 0, 0, 0)" |
+  "direct_expr (hml_pos \<alpha> \<phi>) = (1 + fst (direct_expr \<phi>), 
+                                fst (snd (direct_expr \<phi>)), 
+                                fst (snd (snd (direct_expr \<phi>))), 
+                                fst (snd (snd (snd (direct_expr \<phi>)))), 
+                                fst (snd (snd (snd (snd (direct_expr \<phi>))))), 
+                                snd (snd (snd (snd (snd (direct_expr \<phi>))))))" |
+  "direct_expr (hml_conj I J \<Phi>) = (Sup ((fst \<circ> direct_expr \<circ> \<Phi>) ` I \<union> (fst \<circ> direct_expr \<circ> \<Phi>) ` J), 
+                                    1 + Sup ((fst \<circ> snd \<circ> direct_expr \<circ> \<Phi>) ` I \<union> (fst \<circ> snd \<circ> direct_expr \<circ> \<Phi>) ` J), 
+(Sup ((fst \<circ> direct_expr \<circ> \<Phi>) ` I \<union> (fst \<circ> snd \<circ> snd \<circ> direct_expr \<circ> \<Phi>) ` I \<union> (fst \<circ> snd \<circ> snd \<circ> direct_expr \<circ> \<Phi>) ` J)),
+(Sup (((fst \<circ> direct_expr) ` (pos_r (\<Phi> ` I)))  \<union> (fst \<circ> snd \<circ> snd \<circ> snd \<circ> direct_expr \<circ> \<Phi>) ` I \<union> (fst \<circ> snd \<circ> snd \<circ> snd \<circ> direct_expr \<circ> \<Phi>) ` J)),  
+(Sup ((fst \<circ> snd \<circ> snd \<circ> snd \<circ> snd \<circ> direct_expr \<circ> \<Phi>) ` I \<union> (fst \<circ> snd \<circ> snd \<circ> snd \<circ> snd \<circ> direct_expr \<circ> \<Phi>) ` J \<union> (fst \<circ> direct_expr \<circ> \<Phi>) ` J)), 
+(Sup ((snd \<circ> snd \<circ> snd \<circ> snd \<circ> snd \<circ> direct_expr \<circ> \<Phi>) ` I \<union> ((eSuc \<circ> snd \<circ> snd \<circ> snd \<circ> snd \<circ> snd \<circ> direct_expr \<circ> \<Phi>) ` J))))"
+  by ((meson hml.exhaust), simp+)
+
+text \<open>In order to demonstrate termination of the function, it is necessary to establish that each sequence of recursive function calls reaches a base case. 
+This is accomplished by proving that the relation between process-formula pairs, as defined recursively by the function, is contained within a well-founded relation. 
+A relation \( R \subset X \times X \) is considered well-founded if every non-empty subset \( X' \subset X \) contains a minimal element \( m \) such that \( (x, m) \notin R \) for all \( x \in X' \). 
+A key property of well-founded relations is that all descending chains \( (x_0, x_1, x_2, \ldots) \) (where \( (x_i, x_{i+1}) \in R \)) originating from any element \( x_0 \in X \) are finite. 
+Consequently, this ensures that each sequence of recursive invocations terminates after a finite number of steps. 
+
+These proofs were inspired by the Isabelle formalizations presented in [WEP+16].
+\<close>
+
+inductive_set HML_wf_rel :: "(('a, 's)hml) rel" where
+"\<phi> = \<Phi> i \<and> i \<in> (I \<union> J) \<Longrightarrow> (\<phi>, (hml_conj I J \<Phi>)) \<in> HML_wf_rel" |
+"(\<phi>, (hml_pos \<alpha> \<phi>)) \<in> HML_wf_rel"
+
+lemma HML_wf_rel_is_wf: \<open>wf HML_wf_rel\<close>
+  unfolding wf_def
+proof safe
+  fix P
+  assume assm: "\<forall>x. (\<forall>y. (y, x) \<in> HML_wf_rel \<longrightarrow> P y) \<longrightarrow> P x"
+  show "\<And>\<phi>. P \<phi>" proof-
+    fix \<phi>
+    show "P \<phi>" proof(induction \<phi>)
+    case TT
+    then show ?case 
+      using HML_wf_rel.cases assm by blast
+  next
+    case (hml_pos x1 \<phi>)
+    then show ?case 
+      using HML_wf_rel.cases hml.inject hml.simps assm 
+      by (smt (verit, best))
+  next
+    case (hml_conj x1 x2 x3)
+    then show ?case 
+      using assm
+      by (metis HML_wf_rel.cases hml.inject(2) hml.simps(8) rangeI)
+    qed
+  qed
+qed
+
+lemma pos_r_subs: "pos_r (\<Phi> ` I) \<subseteq> (\<Phi> ` I)"
+  by auto
+
+termination
+  apply rule
+  using HML_wf_rel_is_wf HML_wf_rel.simps Un_iff pos_r_subs by fastforce+
+
+
+
+text \<open>We show that \<open>direct_expr\<close> and \<open>expr\<close> are the same:\<close>
+
+
+(*<*)
+lemma \<^marker>\<open>tag (proof) visible\<close> expr_6_direct_expr_eq:
+  assumes "\<And>x. x \<in> \<Phi> ` I \<Longrightarrow> expr_6 x = snd (snd (snd (snd (snd (direct_expr x)))))"
+  shows "(expr_6 \<circ> \<Phi>) ` I = (snd \<circ> snd \<circ> snd \<circ> snd \<circ> snd \<circ> direct_expr \<circ> \<Phi>) ` I"
+proof -
+  have "(expr_6 \<circ> \<Phi>) ` I = (\<lambda>x. snd (snd (snd (snd (snd (direct_expr (\<Phi> x))))))) ` I"
+    by (simp add: assms)
+  also have "... = (snd \<circ> snd \<circ> snd \<circ> snd \<circ> snd \<circ> direct_expr \<circ> \<Phi>) ` I"
+    by auto
+  finally show ?thesis .
+qed
+
+lemma \<^marker>\<open>tag (proof) visible\<close> expr_6_eSuc_eq:
+  assumes "\<And>x. x \<in> \<Phi> ` J \<Longrightarrow> eSuc (expr_6 x) = eSuc (snd (snd (snd (snd (snd (direct_expr x))))))"
+  shows "((eSuc \<circ> expr_6 \<circ> \<Phi>) ` J) = ((eSuc \<circ> snd \<circ> snd \<circ> snd \<circ> snd \<circ> snd \<circ> direct_expr \<circ> \<Phi>) ` J)"
+proof-
+  have "((eSuc \<circ> expr_6 \<circ> \<Phi>) ` J) = (\<lambda>x. eSuc (snd (snd (snd (snd (snd (direct_expr (\<Phi> x)))))))) ` J"
+    using assms by force
+  also have "... = ((eSuc \<circ> snd \<circ> snd \<circ> snd \<circ> snd \<circ> snd \<circ> direct_expr \<circ> \<Phi>) ` J)"
+    by auto
+  finally show ?thesis.
+qed
+
+lemma \<^marker>\<open>tag (proof) visible\<close> expr_5_dir_eq:
+  assumes "\<forall>x \<in> \<Phi> ` (I \<union> J). expr_5 x = fst (snd (snd (snd (snd (direct_expr x)))))"
+  shows "((expr_5 \<circ> \<Phi>) ` I \<union> (expr_5 \<circ> \<Phi>) ` J) = 
+          ((fst \<circ> snd \<circ> snd \<circ> snd \<circ> snd \<circ> direct_expr \<circ> \<Phi>) ` I \<union> (fst \<circ> snd \<circ> snd \<circ> snd \<circ> snd \<circ> direct_expr \<circ> \<Phi>) ` J)"
+proof-
+  have "((expr_5 \<circ> \<Phi>) ` I \<union> (expr_5 \<circ> \<Phi>) ` J) = (\<lambda>x. fst (snd (snd (snd (snd (direct_expr (\<Phi> x))))))) ` (I \<union> J)"
+    using assms 
+    by auto
+  also have "... = (fst \<circ> snd \<circ> snd \<circ> snd \<circ> snd \<circ> direct_expr \<circ> \<Phi>) ` (I \<union> J)"
+    by auto 
+  also have "... =  ((fst \<circ> snd \<circ> snd \<circ> snd \<circ> snd \<circ> direct_expr \<circ> \<Phi>) ` I \<union> (fst \<circ> snd \<circ> snd \<circ> snd \<circ> snd \<circ> direct_expr \<circ> \<Phi>) ` J)"
+    by blast
+  finally show ?thesis.
+qed
+(*>*)
+
+lemma 
+  shows "expr \<phi> = direct_expr \<phi>"
+proof(induction \<phi>)
+  case TT
+  have "expr TT = (0, 1, 0, 0, 0, 0)" using expr.simps expr_1.simps(1) expr_2.simps(1) expr_3.simps(1) expr_4.simps(1) expr_5.simps(1) expr_6.simps(1)
+    by force
+  then show ?case using direct_expr.simps(1) 
+    by force
+next
+  case (hml_pos \<alpha> \<phi>)
+  hence IH: "(expr_1 \<phi>, expr_2 \<phi>, expr_3 \<phi>, expr_4 \<phi>, expr_5 \<phi>, expr_6 \<phi>) =
+                                (fst (direct_expr \<phi>), 
+                                fst (snd (direct_expr \<phi>)), 
+                                fst (snd (snd (direct_expr \<phi>))), 
+                                fst (snd (snd (snd (direct_expr \<phi>)))), 
+                                fst (snd (snd (snd (snd (direct_expr \<phi>))))), 
+                                snd (snd (snd (snd (snd (direct_expr \<phi>))))))"
+    by auto
+  have expr: "expr (hml_pos \<alpha> \<phi>) = (1 + (expr_1 \<phi>), expr_2 \<phi>, expr_3 \<phi>, expr_4 \<phi>, expr_5 \<phi>, expr_6 \<phi>)"
+    using expr.simps expr_1.simps expr_2.simps expr_3.simps expr_4.simps expr_5.simps expr_6.simps
+    by simp
+  have "direct_expr (hml_pos \<alpha> \<phi>) = 
+                                (1 + fst (direct_expr \<phi>), 
+                                fst (snd (direct_expr \<phi>)), 
+                                fst (snd (snd (direct_expr \<phi>))), 
+                                fst (snd (snd (snd (direct_expr \<phi>)))), 
+                                fst (snd (snd (snd (snd (direct_expr \<phi>))))), 
+                                snd (snd (snd (snd (snd (direct_expr \<phi>))))))"
+    using direct_expr.simps(2) by auto
+  then show ?case using expr IH by force
+next
+  case (hml_conj I J \<Phi>)
+  hence IH: "\<forall>\<phi> \<in> \<Phi> ` I. (expr_1 \<phi>, expr_2 \<phi>, expr_3 \<phi>, expr_4 \<phi>, expr_5 \<phi>, expr_6 \<phi>) =
+                                (fst (direct_expr \<phi>), 
+                                fst (snd (direct_expr \<phi>)), 
+                                fst (snd (snd (direct_expr \<phi>))), 
+                                fst (snd (snd (snd (direct_expr \<phi>)))), 
+                                fst (snd (snd (snd (snd (direct_expr \<phi>))))), 
+                                snd (snd (snd (snd (snd (direct_expr \<phi>))))))"
+        "\<forall>\<phi> \<in> \<Phi> ` J. (expr_1 \<phi>, expr_2 \<phi>, expr_3 \<phi>, expr_4 \<phi>, expr_5 \<phi>, expr_6 \<phi>) =
+                                (fst (direct_expr \<phi>), 
+                                fst (snd (direct_expr \<phi>)), 
+                                fst (snd (snd (direct_expr \<phi>))), 
+                                fst (snd (snd (snd (direct_expr \<phi>)))), 
+                                fst (snd (snd (snd (snd (direct_expr \<phi>))))), 
+                                snd (snd (snd (snd (snd (direct_expr \<phi>))))))"
+    by simp+
+  hence e1: "Sup ((expr_1 \<circ> \<Phi>) ` I \<union> (expr_1 \<circ> \<Phi>) ` J) = Sup ((fst \<circ> direct_expr \<circ> \<Phi>) ` I \<union> (fst \<circ> direct_expr \<circ> \<Phi>) ` J)"
+    by (smt (verit, best) Pair_inject comp_apply image_cong image_eqI)
+  have e2: "1 + Sup ((expr_2 \<circ> \<Phi>) ` I \<union> (expr_2 \<circ> \<Phi>) ` J) = 1 + Sup ((fst \<circ> snd \<circ> direct_expr \<circ> \<Phi>) ` I \<union> (fst \<circ> snd \<circ> direct_expr \<circ> \<Phi>) ` J)"
+    using IH Sup_le_iff 
+    by (smt (verit) Pair_inject comp_apply image_cong image_eqI)
+  have e3: "(Sup ((expr_1 \<circ> \<Phi>) ` I \<union> (expr_3 \<circ> \<Phi>) ` I \<union> (expr_3 \<circ> \<Phi>) ` J)) =
+        (Sup ((fst \<circ> direct_expr \<circ> \<Phi>) ` I \<union> (fst \<circ> snd \<circ> snd \<circ> direct_expr \<circ> \<Phi>) ` I \<union> (fst \<circ> snd \<circ> snd \<circ> direct_expr \<circ> \<Phi>) ` J))"
+    using IH Sup_le_iff 
+    by (smt (verit, ccfv_SIG) Pair_inject comp_apply image_comp image_cong)
+  have e4: "Sup ((expr_1 ` (pos_r (\<Phi> ` I)))  \<union> (expr_4 \<circ> \<Phi>) ` I \<union> (expr_4 \<circ> \<Phi>) ` J) =
+        (Sup (((fst \<circ> direct_expr) ` (pos_r (\<Phi> ` I)))  \<union> (fst \<circ> snd \<circ> snd \<circ> snd \<circ> direct_expr \<circ> \<Phi>) ` I \<union> (fst \<circ> snd \<circ> snd \<circ> snd \<circ> direct_expr \<circ> \<Phi>) ` J))"
+  proof-
+    have sup_pos_r: "\<forall>x \<in> pos_r (\<Phi> ` I). expr_1 x = (fst \<circ> direct_expr) x"
+      using IH 
+      by (metis (no_types, lifting) Diff_iff Pair_inject comp_apply pos_r.simps)
+    hence "Sup (expr_1 ` pos_r (\<Phi> ` I)) = Sup ((fst \<circ> direct_expr) ` pos_r (\<Phi> ` I))"
+      by (meson SUP_cong)
+    have "\<forall>x \<in> \<Phi> ` (I \<union> J). expr_4 x = fst (snd (snd (snd (direct_expr x))))"
+      using IH
+      by blast+
+    hence "Sup ((expr_4 \<circ> \<Phi>) ` I \<union> (expr_4 \<circ> \<Phi>) ` J) = 
+          Sup ((fst \<circ> snd \<circ> snd \<circ> snd \<circ> direct_expr \<circ> \<Phi>) ` I \<union>
+          (fst \<circ> snd \<circ> snd \<circ> snd \<circ> direct_expr \<circ> \<Phi>) ` J)"
+      using SUP_cong by auto
+    then show ?thesis using sup_pos_r 
+      by (metis (no_types, lifting) Sup_union_distrib image_cong inf_sup_aci(6))
+  qed
+  have e5: "(Sup ((expr_5 \<circ> \<Phi>) ` I \<union> (expr_5 \<circ> \<Phi>) ` J \<union> (expr_1 \<circ> \<Phi>) ` J)) =
+  (Sup ((fst \<circ> snd \<circ> snd \<circ> snd \<circ> snd \<circ> direct_expr \<circ> \<Phi>) ` I \<union> (fst \<circ> snd \<circ> snd \<circ> snd \<circ> snd \<circ> direct_expr \<circ> \<Phi>) ` J \<union> (fst \<circ> direct_expr \<circ> \<Phi>) ` J))"
+    using IH
+  proof-
+    have fa_e5: "\<forall>x \<in> \<Phi> ` (I \<union> J). expr_5 x = fst (snd (snd (snd (snd (direct_expr x)))))"
+          "\<forall>x \<in> \<Phi> ` J. expr_1 x = fst (direct_expr x)"
+      using IH 
+      by blast+
+    hence "Sup ((expr_1 \<circ> \<Phi>) ` J )= Sup ((fst \<circ> direct_expr \<circ> \<Phi>) ` J)" 
+      by fastforce
+    have "Sup ((expr_5 \<circ> \<Phi>) ` I \<union> (expr_5 \<circ> \<Phi>) ` J) = 
+          Sup ((fst \<circ> snd \<circ> snd \<circ> snd \<circ> snd \<circ> direct_expr \<circ> \<Phi>) ` I \<union> (fst \<circ> snd \<circ> snd \<circ> snd \<circ> snd \<circ> direct_expr \<circ> \<Phi>) ` J)"
+      using expr_5_dir_eq fa_e5 by force
+    then show ?thesis 
+      using \<open>Sup ((expr_1 \<circ> \<Phi>) ` J )= Sup ((fst \<circ> direct_expr \<circ> \<Phi>) ` J)\<close> 
+      by (simp add: Sup_union_distrib)
+  qed
+
+  have e6: "(Sup ((expr_6 \<circ> \<Phi>) ` I \<union> ((eSuc \<circ> expr_6 \<circ> \<Phi>) ` J))) =
+        (Sup ((snd \<circ> snd \<circ> snd \<circ> snd \<circ> snd \<circ> direct_expr \<circ> \<Phi>) ` I \<union> ((eSuc \<circ> snd \<circ> snd \<circ> snd \<circ> snd \<circ> snd \<circ> direct_expr \<circ> \<Phi>) ` J)))"
+  proof-
+    have "\<forall>x \<in> \<Phi> ` I. expr_6 x = snd (snd (snd (snd (snd (direct_expr x)))))"
+          "\<forall>x \<in> \<Phi> ` J. expr_6 x = snd (snd (snd (snd (snd (direct_expr x)))))"
+      using IH by blast+
+    from this(1) have "((expr_6 \<circ> \<Phi>) ` I) = ((snd \<circ> snd \<circ> snd \<circ> snd \<circ> snd \<circ> direct_expr \<circ> \<Phi>) ` I)"
+      using expr_6_direct_expr_eq by force
+    hence "Sup ((expr_6 \<circ> \<Phi>) ` I) = Sup ((snd \<circ> snd \<circ> snd \<circ> snd \<circ> snd \<circ> direct_expr \<circ> \<Phi>) ` I)"
+      by presburger 
+    have "\<forall>x \<in> \<Phi> ` J. eSuc (expr_6 x) = eSuc (snd (snd (snd (snd (snd (direct_expr x))))))"
+      using \<open>\<forall>x \<in> \<Phi> ` J. expr_6 x = snd (snd (snd (snd (snd (direct_expr x)))))\<close> by simp
+    hence "Sup ((eSuc \<circ> expr_6 \<circ> \<Phi>) ` J) = Sup ((eSuc \<circ> snd \<circ> snd \<circ> snd \<circ> snd \<circ> snd \<circ> direct_expr \<circ> \<Phi>) ` J)"
+      using expr_6_eSuc_eq by auto
+    then show ?thesis using \<open>Sup ((expr_6 \<circ> \<Phi>) ` I) = Sup ((snd \<circ> snd \<circ> snd \<circ> snd \<circ> snd \<circ> direct_expr \<circ> \<Phi>) ` I)\<close>
+      by (simp add: Sup_union_distrib)
+  qed
+
+  then show ?case using e1 e2 e3 e4 e5 e6 by simp
+qed
+
+(*<*)
+end
+(*>*)
