Correspondences.thy
@@ -7,7 +7,7 @@ begin
 
 chapter \<open>Characterizing Equivalences\<close>
 
-text \<open>In this chapter we introduce the modal-logical characterizations $\mathcal{O}_X$ of the various equivalences and link them to the HML sublanguages $\mathcal{O}_{e_X}$ determined 
+text \<open>In this chapter, we introduce the modal-logical characterizations $\mathcal{O}_X$ of the various equivalences and link them to the HML sublanguages $\mathcal{O}_{e_X}$ determined 
 certain by price bounds. The proofs follow the same structure: We first derive the modal characterization of $\mathcal{O}_{e_X}$ and then show that this characterization is equivalent to the corresponding $\mathcal{O}_X$.
 We derive these modal-logical characterizations from (Glaabbeeck). In the appendix we prove for trace equivalence $\mathcal{O}_T$ and bisimilarity $\mathcal{O}_B$ that the modal-logical characterization really captures
 the colloquial definitions via trace sets/the relational definition of bisimilarity.\<close>
